use tiling api in 2dblocktiling

src/lib/poly/gemm/Kuiper.Poly.GEMM.BlockTiling2D.fst
@@ -6,30 +6,18 @@ open Kuiper
 
 #set-options "--z3rlimit 20"
 
-open Kuiper.EMatrix4
+module EM = Kuiper.EMatrix
+
 open Kuiper.Matrix.Reprs.Type
 open Kuiper.Math { even, odd, even_2x, odd_2x1 }
 
-module M = Kuiper.Matrix
-open Kuiper.Matrix {
-  gpu_matrix,
-  gpu_matrix_pts_to,
-  gpu_matrix_pts_to_cell,
-}
+open Kuiper.Matrix
 
-open Kuiper.Matrix4 {
-  gpu_matrix as gpu_matrix4,
-  gpu_matrix_pts_to as m4_pts_to,
-  gpu_matrix_pts_to_cell as m4_pts_to_cell,
-  mlayout4,
-  clayout4
-}
-
-module M4 = Kuiper.Matrix4
 module MS = Kuiper.Spec.GEMM
 module SZ = FStar.SizeT
 module B = Kuiper.Barrier
 
+module R = Kuiper.Matrix.Reprs
 
 open Kuiper.EMatrix { ematrix }
 open Kuiper.VArray {
@@ -37,6 +25,8 @@ open Kuiper.VArray {
   varray_pts_to,
   varray_pts_to_cell
 }
+open Kuiper.TensorCore
+open Kuiper.Matrix.Tiling
 
 (* Description of shared memory used in this kernel. *)
 inline_for_extraction noextract
@@ -49,145 +39,197 @@ let shmems_desc
   SHArray et (bk *^ bn);
 ]
 
-let thread_row_offset
-  (bm bn : szp)
+unfold
+let bid_y
+  (rows cols : erased nat)
+  (bm : erased nat {bm > 0 /\ bm /? rows})
+  (bn : erased nat {bn > 0 /\ bn /? cols})
+  (bid : enatlt (rows/bm * (cols/bn)))
+  : enatlt (rows/bm)
+  =
+    bid / (cols/bn)
+
+unfold
+let bid_x
+  (rows cols : erased nat)
+  (bm : erased nat {bm > 0 /\ bm /? rows})
+  (bn : erased nat {bn > 0 /\ bn /? cols})
+  (bid : enatlt (rows/bm * (cols/bn)))
+  : enatlt (cols/bn)
+  =
+  bid % (cols/bn)
+
+unfold
+let tid_y
+  (bm bn : erased nat)
+  (tm : erased nat {tm > 0 /\ tm /? bm})
+  (tn : erased nat {tn > 0 /\ tn /? bn})
+  (tid : enatlt (bm/tm * (bn/tn)))
+  : enatlt (bm/tm)
+  =
+    tid / (bn/tn)
+
+unfold
+let tid_x
+  (bm bn : erased nat)
+  (tm : erased nat {tm > 0 /\ tm /? bm})
+  (tn : erased nat {tn > 0 /\ tn /? bn})
+  (tid : enatlt (bm/tm * (bn/tn)))
+  : enatlt (bn/tn)
+  =
+    tid % (bn/tn)
+
+inline_for_extraction noextract
+instance concrete_sz_1 : concrete_sz 1 = { x = 1sz }
+
+let block_tile
+  (#et : Type0) {| scalar et |}
+  (#rows #cols : erased nat)
+  (#lC : mlayout rows cols)
+  (gC : gpu_matrix et lC)
+  (bm : szp{bm /? rows})
+  (bn : szp{bn /? cols})
+  (bid : enatlt (rows/bm * (cols/bn)))
+  : gpu_matrix et
+      (subtile_layout lC bm bn
+        (bid_y rows cols bm bn bid) (bid_x rows cols bm bn bid))
+  =
+    gpu_matrix_subtile gC bm bn (bid_y rows cols bm bn bid) (bid_x rows cols bm bn bid)
+
+let thread_tile
+  (#et : Type0) {| scalar et |}
+  (#bm #bn : sz)
+  (#lC_bt : mlayout bm bn)
+  (gC_bt : gpu_matrix et lC_bt)
   (tm : szp{tm /? bm})
   (tn : szp{tn /? bn})
-  (tid : natlt (bm/tm * (bn/tn)))
-  (i : natlt tm)
-  : GTot (natlt bm)
+  (tid : enatlt (bm/tm * (bn/tn)))
+  : gpu_matrix et
+      (subtile_layout lC_bt tm tn
+        (tid_y bm bn tm tn tid) (tid_x bm bn tm tn tid))
   =
-  tid / (bn/tn) * tm + i
+   gpu_matrix_subtile gC_bt tm tn (tid_y bm bn tm tn tid) (tid_x bm bn tm tn tid)
 
 let own_thread_tile
   (#et : Type0) {| scalar et |}
-  (bm bn : szp)
+  (#rows #cols : erased nat)
+  (#lC : mlayout rows cols)
+  (gC : gpu_matrix et lC)
+  (bm : szp{bm /? rows})
+  (bn : szp{bn /? cols})
   (tm : szp{tm /? bm})
   (tn : szp{tn /? bn})
-  (#mrows #mcols : erased nat)
-  (#lC : mlayout4 mrows mcols bm bn)
-  (gC : gpu_matrix4 et lC)
-  (bid : natlt (mrows * mcols))
-  (tid : natlt (bm/tm * (bn/tn)))
+  (bid : enatlt ((rows/bm) * (cols/bn)))
+  (tid : enatlt (bm/tm * (bn/tn)))
   : slprop
-  = (forall+ (i : natlt tm) (j : natlt tn).
-      (exists* v.
-        m4_pts_to_cell gC
-          (bid / mcols) (bid % mcols)
-          (thread_row_offset bm bn tm tn tid i) //(tid / (bn/tn) * tm) + i)
-          ((tid % (bn/tn) * tn) + j)
-          v))
+  = 
+    (exists* em.
+      gpu_matrix_pts_to
+        (thread_tile (block_tile gC bm bn bid) tm tn tid) em)
 
 unfold
 let kpre1
   (#et : Type0) {| scalar et |}
   (comb : binop et)
-  (#bm #bn #bk : szp)
-  (#mrows #mshared #mcols : szp)
+  (#rows #shared #cols : szp)
+  (#lA : mlayout rows shared)
+  (#lB : mlayout shared cols)
+  (#lC : mlayout rows cols)
+  (gA : gpu_matrix et lA)
+  (eA : ematrix et rows shared)
+  (gB : gpu_matrix et lB)
+  (eB : ematrix et shared cols)
+  (gC : gpu_matrix et lC)
+  (bm : szp{bm /? rows})
+  (bn : szp{bn /? cols})
+  (bk : szp{bk /? shared})
   (tm : szp{tm /? bm})
   (tn : szp{tn /? bn})
-  (#lA : mlayout4 mrows   mshared bm bk)
-  (#lB : mlayout4 mshared mcols   bk bn)
-  (#lC : mlayout4 mrows   mcols   bm bn)
-  (gA : gpu_matrix4 et lA)
-  (gB : gpu_matrix4 et lB)
-  (gC : gpu_matrix4 et lC)
-  (eA : ematrix4 et mrows mshared bm bk)
-  (eB : ematrix4 et mshared mcols bk bn)
   (fA fB : perm)
-  (bid : natlt (mrows * mcols))
-  (tid : natlt (bm/tm * (bn/tn)))
+  (bid : enatlt (rows/bm * (cols/bn)))
+  (tid : enatlt (bm/tm * (bn/tn)))
   : slprop
   =
-  (gA |-> Frac (fA /. (mrows * mcols * (bm/tm * (bn/tn)))) eA) **
-  (gB |-> Frac (fB /. (mrows * mcols * (bm/tm * (bn/tn)))) eB) **
-  own_thread_tile bm bn tm tn gC bid tid
+  (gA |-> Frac (fA /. (rows/tm * (cols/tn))) eA) **
+  (gB |-> Frac (fB /. (rows/tm * (cols/tn))) eB) **
+  own_thread_tile gC bm bn tm tn bid tid
 
 unfold
 let kpost1
   (#et : Type0) {| scalar et |}
   (comb : binop et)
-  (#bm #bn #bk : szp)
-  (#mrows #mshared #mcols : szp)
+  (#rows #shared #cols : szp)
+  (#lA : mlayout rows shared)
+  (#lB : mlayout shared cols)
+  (#lC : mlayout rows cols)
+  (gA : gpu_matrix et lA)
+  (eA : ematrix et rows shared)
+  (gB : gpu_matrix et lB)
+  (eB : ematrix et shared cols)
+  (gC : gpu_matrix et lC)
+  (bm : szp{bm /? rows})
+  (bn : szp{bn /? cols})
+  (bk : szp{bk /? shared})
   (tm : szp{tm /? bm})
   (tn : szp{tn /? bn})
-  (#lA : mlayout4 mrows   mshared bm bk)
-  (#lB : mlayout4 mshared mcols   bk bn)
-  (#lC : mlayout4 mrows   mcols   bm bn)
-  (gA : gpu_matrix4 et lA)
-  (gB : gpu_matrix4 et lB)
-  (gC : gpu_matrix4 et lC)
-  (eA : ematrix4 et mrows mshared bm bk)
-  (eB : ematrix4 et mshared mcols bk bn)
   (fA fB : perm)
-  (bid : natlt (mrows * mcols))
-  (tid : natlt (bm/tm * (bn/tn)))
+  (bid : enatlt (rows/bm * (cols/bn)))
+  (tid : enatlt (bm/tm * (bn/tn)))
   : slprop
   =
-  (gA |-> Frac (fA /. (mrows * mcols * (bm/tm * (bn/tn)))) eA) **
-  (gB |-> Frac (fB /. (mrows * mcols * (bm/tm * (bn/tn)))) eB) **
-  own_thread_tile bm bn tm tn gC bid tid
-
-let own_cell
+  (gA |-> Frac (fA /. (rows/tm * (cols/tn))) eA) **
+  (gB |-> Frac (fB /. (rows/tm * (cols/tn))) eB) **
+  own_thread_tile gC bm bn tm tn bid tid
+  
+let own_shmem_cell
   (#et : Type0)
-  (#rows #cols : nat)
+  (#rows #cols : erased nat)
   (#lm : mlayout rows cols)
-  (m : gpu_matrix et lm)
-  (i : natlt rows)
-  (j : natlt cols)
+  (sm : gpu_matrix et lm)
+  (i : enatlt rows)
+  (j : enatlt cols)
   : slprop
-  = exists* v. gpu_matrix_pts_to_cell m i j v
+  = exists* v. gpu_matrix_pts_to_cell sm i j v
 
-let div_ceil (a : nat) (b : pos) = (a + (b-1))/b
+let div_ceil (a : erased nat) (b : pos) = (a + (b-1))/b
 let own_tile_stride_cells
   (#et : Type0)
-  (#rows #cols : nat)
+  (#rows #cols : erased nat)
   (#lm : mlayout rows cols)
-  (m : gpu_matrix et lm)
+  ([@@@mkey] m : gpu_matrix et lm)
   // (em : ematrix et rows cols)
-  (nthr : nat)
-  (tid : natlt nthr)
+  (nthr : erased nat)
+  (tid : enatlt nthr)
   : slprop
   =
+  (* using enatlt here would require enumerable enatlt which is not entirely straightforward *)
   forall+ (it : natlt (div_ceil (rows*cols) nthr)).
-    let flat_idx = tid + (it * nthr) <: nat in
-    let i = flat_idx/cols <: nat in
-    let j = flat_idx%cols <: nat in
+    let flat_idx = tid + (it * nthr) <: erased nat in
+    let i = flat_idx/cols <: erased nat in
+    let j = flat_idx%cols <: erased nat in
       if (i < rows && j < cols)
-      then own_cell m i j
+      then own_shmem_cell m i j
       else emp
 
 inline_for_extraction noextract
-fn cp_tile
+fn cp_matrix
   (#et : Type0) {| scalar et |}
-  (brows bcols : szp)
-  (#mrows #mcols: erased nat)
-  (#slM : mlayout brows bcols)
-  {| clayout slM |}
-  // this should just be a submatrix dst
-  (sM : gpu_matrix et slM)
-  // (#esM : ematrix et brows bcols)
-  (#lA : mlayout4 mrows mcols brows bcols)
-  {| clayout4 lA |}
-  // this should just be a submatrix src
-  (gM : gpu_matrix4 et lA)
+  (rows cols: sz)
+  (#lsrc #ldst : mlayout rows cols)
+  {| clayout lsrc, clayout ldst |}
+  (src : gpu_matrix et lsrc)
+  (#esrc : ematrix et rows cols)
+  (dst : gpu_matrix et ldst)
   (#fM : perm)
-  (#eM : ematrix4 et mrows mcols brows bcols)
-  (mrow : szlt mrows)
-  (mcol : szlt mcols)
   (nthr : sz)
   (tid : szlt nthr)
   preserves
     gpu **
-    pure (SZ.fits (brows * bcols + nthr)) **
-    (gM |-> Frac fM eM)
-  requires
-    own_tile_stride_cells sM nthr tid
-  ensures
-    // exists* eM'.
-    own_tile_stride_cells sM (*eM'*) nthr tid
+    pure (SZ.fits (rows * cols + nthr)) **
+    (src |-> Frac fM esrc) **
+    own_tile_stride_cells dst nthr tid
 {
-  let mlen = brows *^ bcols;
+  let mlen = rows *^ cols;
 
   let mut i : sz = tid;
   while (SZ.(!i <^ mlen))
@@ -196,32 +238,32 @@ fn cp_tile
         pure (vi >= tid) **
         pure (vi % nthr == tid) **
         (i |-> vi) **
-        own_tile_stride_cells sM nthr tid **
+        own_tile_stride_cells dst nthr tid **
         pure (vi < mlen + nthr)
   {
-    let v = M4.gpu_matrix_read gM mrow mcol (!i /^ bcols) (!i %^ bcols);
-    unfold own_tile_stride_cells sM nthr tid;
+    let v = gpu_matrix_read src (!i /^ cols) (!i %^ cols);
+    unfold own_tile_stride_cells dst nthr tid;
 
-    let ite : erased (natlt (div_ceil (brows*bcols) nthr)) = (!i - tid) / nthr;
+    let ite : erased (natlt (div_ceil (rows*cols) nthr)) = (!i - tid) / nthr;
     forevery_extract (reveal ite) _;
 
     rewrite each
-      (((tid + ite * nthr) / bcols < brows) &&
-       ((tid + ite * nthr) % bcols < bcols))
+      (((tid + ite * nthr) / cols < rows) &&
+       ((tid + ite * nthr) % cols < cols))
     as true;
     let vi = !i;
     assert pure (SZ.v vi == (SZ.v tid + ite * SZ.v nthr));
     rewrite each (tid + ite * nthr) as vi;
 
-    unfold own_cell sM (vi / bcols) (vi % bcols);
-    M.gpu_matrix_write_cell sM (!i /^ bcols) (!i %^ bcols) v;
-    fold own_cell sM (vi / bcols) (vi % bcols);
+    unfold own_shmem_cell dst (vi / cols) (vi % cols);
+    gpu_matrix_write_cell dst (!i /^ cols) (!i %^ cols) v;
+    fold own_shmem_cell dst (vi / cols) (vi % cols);
 
     rewrite each SZ.v vi as (tid + ite * nthr);
 
     Pulse.Lib.Trade.elim_trade _ _;
 
-    fold own_tile_stride_cells sM nthr tid;
+    fold own_tile_stride_cells dst nthr tid;
 
     Math.Lemmas.modulo_addition_lemma vi nthr 1;
     i := !i +^ nthr;
@@ -233,8 +275,8 @@ fn cp_tile
 let barrier_p
   (#et : Type0)
   (#bm #bn #bk : szp)
-  (#l1 : full_mlayout bm bk)
-  (#l2 : full_mlayout bk bn)
+  (#l1 : mlayout bm bk)
+  (#l2 : mlayout bk bn)
   (m1 : gpu_matrix et l1)
   (m2 : gpu_matrix et l2)
   (nthr : pos)
@@ -250,8 +292,8 @@ let barrier_p
 let barrier_q
   (#et : Type0)
   (#bm #bn #bk : szp)
-  (#l1 : full_mlayout bm bk)
-  (#l2 : full_mlayout bk bn)
+  (#l1 : mlayout bm bk)
+  (#l2 : mlayout bk bn)
   (m1 : gpu_matrix et l1)
   (m2 : gpu_matrix et l2)
   (nthr : pos)
@@ -268,40 +310,43 @@ let barrier_tok
   (l2 : full_mlayout bk bn)
   (sar1 : gpu_array et (bm * bk))
   (sar2 : gpu_array et (bk * bn))
-  (it : nat)
+  (it : erased nat)
   (nthr : pos)
   (tid : natlt nthr)
   : slprop
   =
-  B.barrier_tok (barrier_p (M.from_array l1 sar1) (M.from_array l2 sar2) nthr)
-                (barrier_q (M.from_array l1 sar1) (M.from_array l2 sar2) nthr)
+  B.barrier_tok (barrier_p (from_array l1 sar1) (from_array l2 sar2) nthr)
+                (barrier_q (from_array l1 sar1) (from_array l2 sar2) nthr)
                 it tid
 
 unfold
 let kpre
   (#et : Type0) {| scalar et |}
   (comb : binop et)
-  (#bm #bn #bk : szp{SZ.fits (bm * bk) /\ SZ.fits (bk * bn)})
-  (#mrows #mshared #mcols : szp)
-  (tm : szp{tm /? bm})
-  (tn : szp{tn /? bn})
+  (#rows #shared #cols : szp)
+  (#lA : mlayout rows shared)
+  (#lB : mlayout shared cols)
+  (#lC : mlayout rows cols)
+  (gA : gpu_matrix et lA)
+  (eA : ematrix et rows shared)
+  (gB : gpu_matrix et lB)
+  (eB : ematrix et shared cols)
+  (gC : gpu_matrix et lC)
+  (bm : szp{bm /? rows})
+  (bn : szp{bn /? cols})
+  (bk : szp{bk /? shared})
+  (#_: squash (SZ.fits (bm * bk) /\ SZ.fits (bk * bn)))
   (slA : full_mlayout bm bk)
   (slB : full_mlayout bk bn)
-  (#lA : mlayout4 mrows   mshared bm bk)
-  (#lB : mlayout4 mshared mcols   bk bn)
-  (#lC : mlayout4 mrows   mcols   bm bn)
-  (gA : gpu_matrix4 et lA)
-  (gB : gpu_matrix4 et lB)
-  (gC : gpu_matrix4 et lC)
-  (eA : ematrix4 et mrows mshared bm bk)
-  (eB : ematrix4 et mshared mcols bk bn)
+  (tm : szp{tm /? bm})
+  (tn : szp{tn /? bn})
   (fA fB : perm)
   (sh : c_shmems (shmems_desc et bm bn bk))
-  (bid : natlt (mrows * mcols))
+  (bid : natlt (rows/bm * (cols/bn)))
   (tid : natlt (bm/tm * (bn/tn)))
   : slprop
   =
-  kpre1 comb tm tn gA gB gC eA eB fA fB bid tid **
+  kpre1 comb gA eA gB eB gC bm bn bk tm tn fA fB bid tid **
   (exists* (x : seq _). fst sh |-> Frac (1.0R /. (bm/tm * (bn/tn))) x) **
   (exists* (x : seq _). fst (snd sh) |-> Frac (1.0R /. (bm/tm * (bn/tn))) x) **
   barrier_tok slA slB (fst sh) (fst (snd sh)) 0 (bm/tm * (bn/tn)) tid
@@ -310,70 +355,80 @@ unfold
 let kpost
   (#et : Type0) {| scalar et |}
   (comb : binop et)
-  (#bm #bn #bk : szp{SZ.fits (bm * bk) /\ SZ.fits (bk * bn)})
-  (#mrows #mshared #mcols : szp)
-  (tm : szp{tm /? bm})
-  (tn : szp{tn /? bn})
+  (#rows #shared #cols : szp)
+  (#lA : mlayout rows shared)
+  (#lB : mlayout shared cols)
+  (#lC : mlayout rows cols)
+  (gA : gpu_matrix et lA)
+  (eA : ematrix et rows shared)
+  (gB : gpu_matrix et lB)
+  (eB : ematrix et shared cols)
+  (gC : gpu_matrix et lC)
+  (bm : szp{bm /? rows})
+  (bn : szp{bn /? cols})
+  (bk : szp{bk /? shared})
+  (#_: squash (SZ.fits (bm * bk) /\ SZ.fits (bk * bn)))
   (slA : full_mlayout bm bk)
   (slB : full_mlayout bk bn)
-  (#lA : mlayout4 mrows   mshared bm bk)
-  (#lB : mlayout4 mshared mcols   bk bn)
-  (#lC : mlayout4 mrows   mcols   bm bn)
-  (gA : gpu_matrix4 et lA)
-  (gB : gpu_matrix4 et lB)
-  (gC : gpu_matrix4 et lC)
-  (eA : ematrix4 et mrows mshared bm bk)
-  (eB : ematrix4 et mshared mcols bk bn)
+  (tm : szp{tm /? bm})
+  (tn : szp{tn /? bn})
   (fA fB : perm)
   (sh : c_shmems (shmems_desc et bm bn bk))
-  (bid : natlt (mrows * mcols))
+  (bid : natlt (rows/bm * (cols/bn)))
   (tid : natlt (bm/tm * (bn/tn)))
   : slprop
   =
-  kpost1 comb tm tn gA gB gC eA eB fA fB bid tid **
+  kpost1 comb gA eA gB eB gC bm bn bk tm tn fA fB bid tid **
   (exists* (x : seq _). fst sh |-> Frac (1.0R /. (bm/tm * (bn/tn))) x) **
   (exists* (x : seq _). fst (snd sh) |-> Frac (1.0R /. (bm/tm * (bn/tn))) x) **
-  barrier_tok slA slB (fst sh) (fst (snd sh)) (2 * mshared) (bm/tm * (bn/tn)) tid
+  barrier_tok slA slB (fst sh) (fst (snd sh)) (2 * (shared/bk)) (bm/tm * (bn/tn)) tid
 
 inline_for_extraction noextract
 fn populate_shmem
   (#et : Type0) {| scalar et |}
-  (bm bn bk : szp)
-  (#mrows #mshared #mcols : erased nat)
+  (#rows #shared #cols : erased nat)
+  (bm : szp{bm /? rows})
+  (bn : szp{bn /? cols})
+  (bk : szp{bk /? shared})
   (tm : szp{tm /? bm})
   (tn : szp{tn /? bn})
-  (#slA : full_mlayout bm bk) {| clayout slA |}
-  (#slB : full_mlayout bk bn) {| clayout slB |}
+  (#slA : mlayout bm bk) {| clayout slA |}
+  (#slB : mlayout bk bn) {| clayout slB |}
   (sA : gpu_matrix et slA)
   (sB : gpu_matrix et slB)
-  (#lA : mlayout4 mrows   mshared bm bk)
-  (#lB : mlayout4 mshared mcols   bk bn)
-  {| clA: clayout4 lA, clayout4 lB |}
-  // should be gpu_matrix and just pointers to the tiles
-  (gA : gpu_matrix4 et lA)
-  (gB : gpu_matrix4 et lB)
+  (#lA : mlayout rows shared) {| clayout lA |}
+  (#lB : mlayout shared cols) {| clayout lB |}
+  (gA : gpu_matrix et lA)
+  (#eA : ematrix et rows shared)
+  (gB : gpu_matrix et lB)
   (#fA #fB : perm)
-  (#eA : ematrix4 et mrows   mshared bm bk)
-  (#eB : ematrix4 et mshared mcols   bk bn)
-  (mrow : szlt mrows)
-  (mk : szlt mshared)
-  (mcol : szlt mcols)
+  (#eB : ematrix et shared cols)
   (#_ : squash (SZ.fits (bm*bk + bm/tm*(bn/tn))))
   (#_ : squash (SZ.fits (bk*bn + bm/tm*(bn/tn))))
+  (tile_row : szlt (rows/bm))
+  (tile_shared : szlt (shared/bk))
+  (tile_col : szlt (cols/bn))
   (tid : szlt (bm/^tm *^ (bn/^tn)))
   preserves
     gpu **
     (gA |-> Frac fA eA) **
     (gB |-> Frac fB eB) **
+    thread_id (bm/^tm *^ (bn/^tn)) tid **
     own_tile_stride_cells sA (bm/tm * (bn/tn)) tid **
     own_tile_stride_cells sB (bm/tm * (bn/tn)) tid
 {
-  let nthr = bm /^ tm *^ (bn /^ tn);  assert (rewrites_to nthr (bm /^ tm *^ (bn /^ tn)));
-  cp_tile bm bk sA gA mrow mk nthr tid;
-  cp_tile bk bn sB gB mk mcol nthr tid;
+  let tileA = gpu_matrix_extract_tile' gA bm bk tile_row tile_shared;
+  cp_matrix bm bk tileA sA (get_bdim()) tid;
+
+  let tileB = gpu_matrix_extract_tile' gB bk bn tile_shared tile_col;
+  cp_matrix bk bn tileB sB (get_bdim()) tid;
+
+  ambig_trade_elim ();
+  ambig_trade_elim ();
   ();
 }
 
+// #push-options "--debug SMTFail --split_queries always --print_implicits"
 inline_for_extraction noextract
 fn subproducts2d
   (#et : Type0) {| scalar et |}
@@ -382,8 +437,8 @@ fn subproducts2d
   (tn : szp{tn /? bn})
   (rAcol rBrow rchProd: array et)
   (#vrAcol #vrBrow #vrchProd : erased (seq et))
-  (#l1 : full_mlayout bm bk) {| clayout l1 |}
-  (#l2 : full_mlayout bk bn) {| clayout l2 |}
+  (#l1 : mlayout bm bk) {| clayout l1 |}
+  (#l2 : mlayout bk bn) {| clayout l2 |}
   (gA : gpu_matrix et l1)
   (gB : gpu_matrix et l2)
   (#eA : ematrix et bm bk)
@@ -431,7 +486,10 @@ fn subproducts2d
           (i0 |-> vi) **
           (rAcol |-> vrAcol)
     {
-      let va = M.gpu_matrix_read gA (arow *^ tm +^ !i0) !dotIdx;
+      (* get rid of a few non-linear arithmetic expressions *)
+      let a_tile = gpu_matrix_extract_tile' gA tm 1 arow !dotIdx;
+      let va = gpu_matrix_read a_tile !i0 0sz;
+      ambig_trade_elim ();
       rAcol.(!i0) <- va;
 
       i0 := !i0 +^ 1sz;
@@ -444,7 +502,9 @@ fn subproducts2d
           (i1 |-> vi) **
           (rBrow |-> vrBrow)
     {
-      let vb = M.gpu_matrix_read gB !dotIdx (bcol *^ tn +^ !i1);
+      let b_tile = gpu_matrix_extract_tile' gB 1 tn !dotIdx bcol;
+      let vb = gpu_matrix_read b_tile 0sz !i1;
+      ambig_trade_elim ();
       rBrow.(!i1) <- vb;
 
       i1 := !i1 +^ 1sz;
@@ -464,6 +524,7 @@ fn subproducts2d
             (resIdxN |-> vresIdxN) **
             (rchProd |-> vrchProd)
       {
+        (* works on arrays and therefore does not have the nice matrix abstraction *)
         let ra = rAcol.(!resIdxM);
         let rb = rBrow.(!resIdxN);
         let iM = !resIdxM;
@@ -487,80 +548,65 @@ inline_for_extraction noextract
 fn epilogue
   (#et : Type0) {| scalar et |}
   (comb : binop et)
-  (bm bn bk : szp)
-  (#mrows #mcols : szp)
+  (#rows #cols : sz)
+  (bm : szp{bm /? rows})
+  (bn : szp{bn /? cols})
   (tm : szp{tm /? bm})
   (tn : szp{tn /? bn})
   (rchProd: array et)
-  (#lC : mlayout4 mrows   mcols   bm bn)
-  {| clayout4 lC |}
-  (gC : gpu_matrix4 et lC)
-  (bid : szlt (mrows * mcols))
+  (#lC : mlayout rows cols)
+  {| clayout lC |}
+  (gC : gpu_matrix et lC)
+  // (#_ : squash (SZ.fits (bm/tm * (bn/tn))))
+  (bid : szlt (rows/bm * (cols/bn)))
   (tid : szlt (bm/tm * (bn/tn)))
   requires
     gpu **
-    own_thread_tile bm bn tm tn gC bid tid **
+    own_thread_tile gC bm bn tm tn bid tid **
     (exists* vrchProd.
       pure (Seq.length vrchProd == tm * tn) **
       (rchProd |-> vrchProd))
   ensures
     gpu **
-    own_thread_tile bm bn tm tn gC bid tid **
+    own_thread_tile gC bm bn tm tn bid tid **
     (exists* vrchProd'.
       pure (Seq.length vrchProd' == tm * tn) **
       (rchProd |-> vrchProd'))
 {
-  unfold own_thread_tile bm bn tm tn gC bid tid;
-
-  let mrow = bid /^ mcols;
-  let mcol = bid %^ mcols;
-  let tRowOff = tid /^ (bn /^ tn) *^ tm;
-  let tColOff = tid %^ (bn /^ tn) *^ tn;
+  unfold own_thread_tile gC bm bn tm tn bid tid;
+  let t_tile = thread_tile (block_tile gC bm bn bid) tm tn tid;
+  assert (rewrites_to t_tile (thread_tile (block_tile gC bm bn bid) tm tn tid));
 
   let mut resIdxM = 0sz;
   while (SZ.(!resIdxM <^ tm))
     invariant
-      exists* (vresIdxM : sz{vresIdxM <= tm}) (vrchProd : lseq et (tm*tn)).
+      exists* (vresIdxM : sz{vresIdxM <= tm}) (vrchProd : lseq et (tm*tn)) (v : ematrix et tm tn).
         (resIdxM |-> vresIdxM) **
-        (rchProd |-> vrchProd)
+        (rchProd |-> vrchProd) **
+        gpu_matrix_pts_to t_tile v
   {
     let mut resIdxN = 0sz;
     while (SZ.(!resIdxN <^ tn))
       invariant
-        exists* (vresIdxN : sz{vresIdxN <= tn}) (vrchProd : lseq et (tm*tn)).
+        exists* (vresIdxN : sz{vresIdxN <= tn}) (vrchProd : lseq et (tm*tn)) (v : ematrix et tm tn).
           (resIdxN |-> vresIdxN) **
-          (rchProd |-> vrchProd)
+          (rchProd |-> vrchProd) **
+          gpu_matrix_pts_to t_tile v
+
     {
-      let vresIdxM = !resIdxM;
-      let vresIdxN = !resIdxN;
-
-      (* get separate access to the thread's current cell in gC *)
-      forevery_extract_2 #(natlt tm) #_ #(natlt tn) (SZ.v vresIdxM) (SZ.v vresIdxN) _;
-
-      (* tame the SMT solver *)
-      assert pure(SZ.v tid / (SZ.v bn / SZ.v tn) * SZ.v tm == tRowOff);
-      assert pure(SZ.v tid % (SZ.v bn / SZ.v tn) * SZ.v tn == tColOff);
-
-      assert pure (thread_row_offset bm bn tm tn tid vresIdxM == tid/(bn/tn)*tm + vresIdxM ==> tid/(bn/tn)*tm + vresIdxM < bm);
-      (* read the current cell in gC *)
-      with bi0 bj0 i0 j0 v0.
-      rewrite M4.gpu_matrix_pts_to_cell gC bi0  bj0  i0   j0   v0
-          as M4.gpu_matrix_pts_to_cell gC mrow mcol (tRowOff + vresIdxM) (tColOff + vresIdxN) v0;
-      let v0 = M4.gpu_matrix_read_cell gC mrow mcol (tRowOff +^ vresIdxM) (tColOff +^ vresIdxN);
+      let v0 = gpu_matrix_read t_tile !resIdxM !resIdxN;
 
       (* add the new result in the register cache to the value from gC and overwrite the the cell in gC *)
       open Pulse.Lib.Array;
+      // all obvious but without the asserts the next line fails
+      assert pure (SZ.fits (tm * tn));
+      assert pure (SZ.fits ((tm-1) * tn + tn));
+      with vrchProd. assert Pulse.Lib.Array.Core.pts_to rchProd vrchProd;
+      assert pure (Seq.length vrchProd == tm * tn);
       let v1 = rchProd.(!resIdxM *^ tn +^ !resIdxN);
       let v' = comb v0 v1;
-      M4.gpu_matrix_write_cell gC mrow mcol (tRowOff +^ vresIdxM) (tColOff +^ vresIdxN) v';
 
-      (* return separate access to the thread's current cell in gC *)
-      rewrite each (SZ.v mrow) as (bid/mcols);
-      rewrite each (SZ.v mcol) as (bid%mcols);
-      rewrite each (SZ.v tRowOff) as (tid/(bn/tn) * tm);
-      rewrite each (tid/(bn/tn) * tm + (SZ.v vresIdxM)) as thread_row_offset bm bn tm tn tid (SZ.v vresIdxM);
-      rewrite each (SZ.v tColOff) as (tid%(bn/tn) * tn);
-      Pulse.Lib.Trade.elim_trade _ _;
+      gpu_matrix_write t_tile !resIdxM !resIdxN v';
 
       resIdxN := !resIdxN +^ 1sz;
     };
@@ -568,7 +614,8 @@ fn epilogue
     resIdxM := !resIdxM +^ 1sz;
   };
 
-  fold own_thread_tile bm bn tm tn gC bid tid;
+  // rewrite each t_tile as thread_tile (block_tile gC bm bn bid) tm tn tid;
+  fold own_thread_tile gC bm bn tm tn bid tid;
   ()
 }
 
@@ -576,40 +623,42 @@ inline_for_extraction noextract
 fn kf
   (#et : Type0) {| scalar et |}
   (comb : binop et)
-  (#bm #bn #bk : szp)
-  (#mrows #mshared #mcols : szp)
+  (#rows #shared #cols : szp)
+  (#lA : mlayout rows shared)
+  (#lB : mlayout shared cols)
+  (#lC : mlayout rows cols)
+  {| clayout lA, clayout lB, clayout lC |}
+  (gA : gpu_matrix et lA)
+  (#eA : ematrix et rows shared)
+  (gB : gpu_matrix et lB)
+  (#eB : ematrix et shared cols)
+  (gC : gpu_matrix et lC)
+  (bm : szp{bm /? rows})
+  (bn : szp{bn /? cols})
+  (bk : szp{bk /? shared})
+  (#_: squash (SZ.fits (bm * bk) /\ SZ.fits (bk * bn)))
+  (slA : full_mlayout bm bk)
+  (slB : full_mlayout bk bn)
+  {| clayout slA, clayout slB |}
   (tm : szp{tm /? bm})
   (tn : szp{tn /? bn})
   (#_ : squash (SZ.fits (bm*bk + bm/tm*(bn/tn))))
   (#_ : squash (SZ.fits (bk*bn + bm/tm*(bn/tn))))
-  (slA : full_mlayout bm bk)
-  (slB : full_mlayout bk bn)
-  {| clayout slA, clayout slB |}
-  (#lA : mlayout4 mrows   mshared bm bk)
-  (#lB : mlayout4 mshared mcols   bk bn)
-  (#lC : mlayout4 mrows   mcols   bm bn)
-  {| clayout4 lA, clayout4 lB, clayout4 lC |}
-  (gA : gpu_matrix4 et lA)
-  (#fA : perm)
-  (gB : gpu_matrix4 et lB)
-  (#fB : perm)
-  (gC : gpu_matrix4 et lC)
-  (#eA : ematrix4 et mrows mshared bm bk)
-  (#eB : ematrix4 et mshared mcols bk bn)
+  (#fA #fB : perm)
   (sh : c_shmems (shmems_desc et bm bn bk))
-  (bid : szlt (mrows * mcols))
+  (bid : szlt (rows/bm * (cols/bn)))
   (tid : szlt (bm/tm * (bn/tn)))
   ()
   requires
     gpu **
-    kpre comb tm tn slA slB gA gB gC eA eB fA fB sh bid tid **
+    kpre comb gA eA gB eB gC bm bn bk slA slB tm tn fA fB sh bid tid **
     thread_id (bm/tm * (bn/tn)) tid **
-    block_id (mrows * mcols) bid
+    block_id (rows/bm * (cols/bn)) bid
   ensures
     gpu **
-    kpost comb tm tn slA slB gA gB gC eA eB fA fB sh bid tid **
+    kpost comb gA eA gB eB gC bm bn bk slA slB tm tn fA fB sh bid tid **
     thread_id (bm/tm * (bn/tn)) tid **
-    block_id (mrows * mcols) bid
+    block_id (rows/bm * (cols/bn)) bid
 {
   let sarA : gpu_array et (bm * bk) = fst sh;
   let sarB : gpu_array et (bk * bn) = fst (snd sh);
@@ -621,16 +670,19 @@ fn kf
 
   unfold barrier_tok slA slB sarA sarB 0 (bm/tm * (bn/tn)) tid;
 
-  M.gpu_matrix_abs' slA sarA;
-  let sA = M.from_array slA sarA;
-  rewrite each M.from_array slA sarA as sA;
+  gpu_matrix_abs' slA sarA;
+  let sA = from_array slA sarA;
+  rewrite each from_array slA sarA as sA;
 
-  M.gpu_matrix_abs' slB sarB;
-  let sB = M.from_array slB sarB;
-  rewrite each M.from_array slB sarB as sB;
+  gpu_matrix_abs' slB sarB;
+  let sB = from_array slB sarB;
+  rewrite each from_array slB sarB as sB;
 
-  let mrow = bid /^ mcols;
-  let mcol = bid %^ mcols;
+  let num_k_tiles = shared /^ bk;
+  let num_n_tiles = cols /^ bn;
+  let mrow = bid /^ num_n_tiles;
+  let mcol = bid %^ num_n_tiles;
+
   let threadRow = tid /^ (bn/^tn);
   let threadCol = tid %^ (bn/^tn);
 
@@ -640,19 +692,16 @@ fn kf
   let mut rchProd : Pulse.Lib.Array.array et = [| zero #et #_ ; tm*^tn |];
 
   let mut bkIdx  : sz = 0sz;
-  while (SZ.(!bkIdx <^ mshared))
-    invariant b.
-      exists* (vbkIdx : SZ.t{vbkIdx <= mshared}) (vrAcol : lseq et tm) (vrBrow : lseq et tn) (vrchProd : lseq et (tm*tn)).
-        pure (b == (SZ.v vbkIdx < mshared)) **
+  while (SZ.(!bkIdx <^ num_k_tiles))
+    invariant
+      exists* (vbkIdx : SZ.t{vbkIdx <= num_k_tiles}) (vrAcol : lseq et tm) (vrBrow : lseq et tn) (vrchProd : lseq et (tm*tn)).
         (bkIdx |-> vbkIdx) **
         (rAcol |-> vrAcol) **
         (rBrow |-> vrBrow) **
         (rchProd |-> vrchProd) **
-        (gA |-> Frac (fA /. (mrows * mcols * (bm/tm * (bn/tn)))) eA) **
-        (gB |-> Frac (fB /. (mrows * mcols * (bm/tm * (bn/tn)))) eB) **
-        (exists* (x : ematrix _ _ _). sA |-> Frac (1.0R /. (bm/tm * (bn/tn))) x) **
-        (exists* (x : ematrix _ _ _). sB |-> Frac (1.0R /. (bm/tm * (bn/tn))) x) **
-        B.barrier_tok (barrier_p sA sB (bm/tm * (bn/tn))) (barrier_q sA sB (bm/tm * (bn/tn))) (2 * vbkIdx) tid **
+        (exists* (x : ematrix _ _ _). sA |-> Frac (1.0R /. ((bm/tm*(bn/tn)))) x) **
+        (exists* (x : ematrix _ _ _). sB |-> Frac (1.0R /. ((bm/tm*(bn/tn)))) x) **
+        B.barrier_tok (barrier_p sA sB ((bm/tm*(bn/tn)))) (barrier_q sA sB ((bm/tm*(bn/tn)))) (2 * vbkIdx) tid **
         gpu
   {
     (* This assert should not be needed. I don't know what effect it even has. *)
@@ -696,48 +745,52 @@ fn kf
     bkIdx := !bkIdx +^ 1sz;
   };
 
-  epilogue comb bm bn bk tm tn rchProd gC bid tid;
+  epilogue comb bm bn tm tn rchProd gC bid tid;
 
-  M.gpu_matrix_concr sA; rewrite each M.core sA as sarA;
-  M.gpu_matrix_concr sB; rewrite each M.core sB as sarB;
+  gpu_matrix_concr sA; rewrite each core sA as sarA;
+  gpu_matrix_concr sB; rewrite each core sB as sarB;
 
-  fold barrier_tok slA slB sarA sarB (2 * mshared) (bm/tm * (bn/tn)) tid;
+  fold barrier_tok slA slB sarA sarB (2 * num_k_tiles) (bm/tm * (bn/tn)) tid;
 
   rewrite each sarA as fst sh;
   rewrite each sarB as fst (snd sh);
   ()
 }
 
-
+#push-options "--z3rlimit 20"
 ghost
 fn setup
   (#et : Type0) {| scalar et |}
   (comb : binop et)
-  (bm bn bk : szp{SZ.fits (bm * bk) /\ SZ.fits (bk * bn)})
-  (#mrows #mshared #mcols : szp)
+  (#rows #shared #cols : szp)
+  (#lA : mlayout rows shared)
+  (#lB : mlayout shared cols)
+  (#lC : mlayout rows cols)
+  {| clayout lA, clayout lB, clayout lC |}
+  (gA : gpu_matrix et lA)
+  (eA : ematrix et rows shared)
+  (gB : gpu_matrix et lB)
+  (eB : ematrix et shared cols)
+  (gC : gpu_matrix et lC)
+  (eC : ematrix et rows cols)
+  (bm : szp{bm /? rows})
+  (bn : szp{bn /? cols})
+  (bk : szp{bk /? shared})
+  // (#_: squash (SZ.fits (bm * bk) /\ SZ.fits (bk * bn)))
+  (#_: squash (SZ.fits (bm * bn)))
+  (#_: squash (SZ.fits (rows * cols)))
   (tm : szp{tm /? bm})
   (tn : szp{tn /? bn})
-  (#lA : mlayout4 mrows   mshared bm bk)
-  (#lB : mlayout4 mshared mcols   bk bn)
-  (#lC : mlayout4 mrows   mcols   bm bn)
-  {| clayout4 lA, clayout4 lB, clayout4 lC |}
-  (gA : gpu_matrix4 et lA)
-  (#fA : perm)
-  (gB : gpu_matrix4 et lB)
-  (#fB : perm)
-  (gC : gpu_matrix4 et lC)
-  (#eA : ematrix4 et mrows mshared bm bk)
-  (#eB : ematrix4 et mshared mcols bk bn)
-  (#eC : ematrix4 et mrows mcols bm bn)
+  (fA fB : perm)
   ()
   requires
     (gA |-> Frac fA eA) **
     (gB |-> Frac fB eB) **
     (gC |-> eC)
   ensures
-    (forall+ (bid : natlt (mrows *^ mcols))
-             (tid : natlt (bm /^ tm *^ (bn /^ tn))).
-      kpre1 comb tm tn gA gB gC eA eB fA fB bid tid) **
+    (forall+ (bid : natlt (rows/^bm *^ (cols/^bn)))
+             (tid : natlt (bm/^tm *^ (bn/^tn))).
+      kpre1 comb gA eA gB eB gC bm bn bk tm tn fA fB bid tid) **
     emp (* frame *)
 {
   admit();
@@ -747,36 +800,40 @@ ghost
 fn block_setup
   (#et : Type0) {| scalar et |}
   (comb : binop et)
-  (bm bn bk : szp{SZ.fits (bm * bk) /\ SZ.fits (bk * bn)})
-  (#mrows #mshared #mcols : szp)
-  (tm : szp{tm /? bm})
-  (tn : szp{tn /? bn})
+  (#rows #shared #cols : szp)
+  (#lA : mlayout rows shared)
+  (#lB : mlayout shared cols)
+  (#lC : mlayout rows cols)
+  (gA : gpu_matrix et lA)
+  (eA : ematrix et rows shared)
+  (gB : gpu_matrix et lB)
+  (eB : ematrix et shared cols)
+  (gC : gpu_matrix et lC)
+  (eC : ematrix et rows cols)
+  (bm : szp{bm /? rows})
+  (bn : szp{bn /? cols})
+  (bk : szp{bk /? shared})
+  // (#_: squash (SZ.fits (bm * bk) /\ SZ.fits (bk * bn)))
+  (#_: squash (SZ.fits (bm * bn)))
+  (#_: squash (SZ.fits (rows * cols)))
   (slA : full_mlayout bm bk)
   (slB : full_mlayout bk bn)
-  (#lA : mlayout4 mrows   mshared bm bk)
-  (#lB : mlayout4 mshared mcols   bk bn)
-  (#lC : mlayout4 mrows   mcols   bm bn)
-  {| clayout4 lA, clayout4 lB, clayout4 lC |}
-  (gA : gpu_matrix4 et lA)
-  (#fA : perm)
-  (gB : gpu_matrix4 et lB)
-  (#fB : perm)
-  (gC : gpu_matrix4 et lC)
-  (#eA : ematrix4 et mrows mshared bm bk)
-  (#eB : ematrix4 et mshared mcols bk bn)
-  (#eC : ematrix4 et mrows mcols bm bn)
+  {| clayout slA, clayout slB |}
+  (tm : szp{tm /? bm})
+  (tn : szp{tn /? bn})
+  (fA fB : perm)
   (sh : c_shmems (shmems_desc et bm bn bk))
-  (bid : natlt (mrows *^ mcols))
+  (bid : natlt (rows/^bm *^ (cols/^bn)))
   ()
   requires
-    block_setup_tok (bm /^ tm *^ (bn /^ tn)) **
+    block_setup_tok (bm/^tm *^ (bn/^tn)) **
     live_c_shmems sh **
-    (forall+ (tid : natlt (bm/^tm *^ (bn /^ tn))).
-      kpre1 comb tm tn gA gB gC eA eB fA fB bid tid)
+    (forall+ (tid : natlt (bm/^tm *^ (bn/^tn))).
+      kpre1 comb gA eA gB eB gC bm bn bk tm tn fA fB bid tid)
   ensures
-    block_setup_tok (bm/^tm *^ (bn /^ tn)) **
-    (forall+ (tid : natlt (bm/^tm *^ (bn /^ tn))).
-      kpre comb tm tn slA slB gA gB gC eA eB fA fB sh bid tid) **
+    block_setup_tok (bm/^tm *^ (bn/^tn)) **
+    (forall+ (tid : natlt (bm/^tm *^ (bn/^tn))).
+      kpre comb gA eA gB eB gC bm bn bk slA slB tm tn fA fB sh bid tid) **
     emp (* frame *)
 {
   admit();
@@ -786,35 +843,39 @@ ghost
 fn block_teardown
   (#et : Type0) {| scalar et |}
   (comb : binop et)
-  (bm bn bk : szp{SZ.fits (bm * bk) /\ SZ.fits (bk * bn)})
-  (#mrows #mshared #mcols : szp)
-  (tm : szp{tm /? bm})
-  (tn : szp{tn /? bn})
+  (#rows #shared #cols : szp)
+  (#lA : mlayout rows shared)
+  (#lB : mlayout shared cols)
+  (#lC : mlayout rows cols)
+  (gA : gpu_matrix et lA)
+  (eA : ematrix et rows shared)
+  (gB : gpu_matrix et lB)
+  (eB : ematrix et shared cols)
+  (gC : gpu_matrix et lC)
+  (eC : ematrix et rows cols)
+  (bm : szp{bm /? rows})
+  (bn : szp{bn /? cols})
+  (bk : szp{bk /? shared})
+  // (#_: squash (SZ.fits (bm * bk) /\ SZ.fits (bk * bn)))
+  (#_: squash (SZ.fits (rows * cols)))
+  (#_: squash (SZ.fits (bm * bn)))
   (slA : full_mlayout bm bk)
   (slB : full_mlayout bk bn)
-  (#lA : mlayout4 mrows   mshared bm bk)
-  (#lB : mlayout4 mshared mcols   bk bn)
-  (#lC : mlayout4 mrows   mcols   bm bn)
-  {| clayout4 lA, clayout4 lB, clayout4 lC |}
-  (gA : gpu_matrix4 et lA)
-  (#fA : perm)
-  (gB : gpu_matrix4 et lB)
-  (#fB : perm)
-  (gC : gpu_matrix4 et lC)
-  (#eA : ematrix4 et mrows mshared bm bk)
-  (#eB : ematrix4 et mshared mcols bk bn)
-  (#eC : ematrix4 et mrows mcols bm bn)
+  {| clayout slA, clayout slB |}
+  (tm : szp{tm /? bm})
+  (tn : szp{tn /? bn})
+  (fA fB : perm)
   (sh : c_shmems (shmems_desc et bm bn bk))
-  (bid : natlt (mrows *^ mcols))
+  (bid : natlt (rows/^bm *^ (cols/^bn)))
   ()
   requires
-    (forall+ (tid : natlt (bm/^tm *^ (bn /^ tn))).
-      kpost comb tm tn slA slB gA gB gC eA eB fA fB sh bid tid) **
+    (forall+ (tid : natlt (bm/^tm *^ (bn/^tn))).
+      kpost comb gA eA gB eB gC bm bn bk slA slB tm tn fA fB sh bid tid) **
     emp (* frame *)
   ensures
     live_c_shmems sh **
-    (forall+ (tid : natlt (bm/^tm *^ (bn /^ tn))).
-      kpost1 comb tm tn gA gB gC eA eB fA fB bid tid)
+    (forall+ (tid : natlt (bm/^tm *^ (bn/^tn))).
+      kpost1 comb gA eA gB eB gC bm bn bk tm tn fA fB bid tid)
 {
   admit();
 }
@@ -823,27 +884,29 @@ ghost
 fn teardown
   (#et : Type0) {| scalar et |}
   (comb : binop et)
-  (bm bn bk : szp{SZ.fits (bm * bk) /\ SZ.fits (bk * bn)})
-  (#mrows #mshared #mcols : szp)
+  (#rows #shared #cols : szp)
+  (#lA : mlayout rows shared)
+  (#lB : mlayout shared cols)
+  (#lC : mlayout rows cols)
+  (gA : gpu_matrix et lA)
+  (eA : ematrix et rows shared)
+  (gB : gpu_matrix et lB)
+  (eB : ematrix et shared cols)
+  (gC : gpu_matrix et lC)
+  (eC : ematrix et rows cols)
+  (bm : szp{bm /? rows})
+  (bn : szp{bn /? cols})
+  (bk : szp{bk /? shared})
+  (#_: squash (SZ.fits (rows * cols)))
+  (#_: squash (SZ.fits (bm * bn)))
   (tm : szp{tm /? bm})
   (tn : szp{tn /? bn})
-  (#lA : mlayout4 mrows   mshared bm bk)
-  (#lB : mlayout4 mshared mcols   bk bn)
-  (#lC : mlayout4 mrows   mcols   bm bn)
-  {| clayout4 lA, clayout4 lB, clayout4 lC |}
-  (gA : gpu_matrix4 et lA)
-  (#fA : perm)
-  (gB : gpu_matrix4 et lB)
-  (#fB : perm)
-  (gC : gpu_matrix4 et lC)
-  (#eA : ematrix4 et mrows mshared bm bk)
-  (#eB : ematrix4 et mshared mcols bk bn)
-  (#eC : ematrix4 et mrows mcols bm bn)
+  (fA fB : perm)
   ()
   requires
-    (forall+ (bid : natlt (mrows *^ mcols))
-             (tid : natlt (bm /^ tm *^ (bn /^ tn))).
-      kpost1 comb tm tn gA gB gC eA eB fA fB bid tid) **
+    (forall+ (bid : natlt (rows/^bm *^ (cols/^bn)))
+             (tid : natlt (bm/^tm *^ (bn/^tn))).
+      kpre1 comb gA eA gB eB gC bm bn bk tm tn fA fB bid tid) **
     emp (* frame *)
   ensures
     (gA |-> Frac fA eA) **
@@ -859,95 +922,103 @@ fn teardown
     // (fun (bid, tid) -> kpost1 comb tile gA gB gC eA eB 1.0R bid tid);
   admit();
 }
+#pop-options
 
 inline_for_extraction noextract
 let mk_kernel
   (#et : Type0) {| scalar et |}
   (comb : binop et)
-  (bm bn bk : szp)
-  (#mrows #mshared #mcols : szp)
-  (tm : szp{tm /? bm})
-  (tn : szp{tn /? bn})
-  (#_ : squash (SZ.fits (bm*bk + bm/tm*(bn/tn))))
-  (#_ : squash (SZ.fits (bk*bn + bm/tm*(bn/tn))))
+  (#rows #shared #cols : szp)
+  (#lA : mlayout rows shared)
+  (#lB : mlayout shared cols)
+  (#lC : mlayout rows cols)
+  {| clayout lA, clayout lB, clayout lC |}
+  (gA : gpu_matrix et lA)
+  (#eA : ematrix et rows shared)
+  (gB : gpu_matrix et lB)
+  (#eB : ematrix et shared cols)
+  (gC : gpu_matrix et lC)
+  (#eC : ematrix et rows cols)
+  (bm : szp{bm /? rows})
+  (bn : szp{bn /? cols})
+  (bk : szp{bk /? shared})
+  (#_: squash (SZ.fits (bm * bk) /\ SZ.fits (bk * bn)))
   (slA : full_mlayout bm bk)
   (slB : full_mlayout bk bn)
   {| clayout slA, clayout slB |}
-  (#lA : mlayout4 mrows   mshared bm bk)
-  (#lB : mlayout4 mshared mcols   bk bn)
-  (#lC : mlayout4 mrows   mcols   bm bn)
-  {| clayout4 lA, clayout4 lB, clayout4 lC |}
-  (gA : gpu_matrix4 et lA)
-  (#fA : perm)
-  (gB : gpu_matrix4 et lB)
-  (#fB : perm)
-  (gC : gpu_matrix4 et lC)
-  (#eA : ematrix4 et mrows mshared bm bk)
-  (#eB : ematrix4 et mshared mcols bk bn)
-  (#eC : ematrix4 et mrows mcols bm bn)
-  (_ : squash (mrows * mcols <= max_blocks
+  (tm : szp{tm /? bm})
+  (tn : szp{tn /? bn})
+  (#fA #fB : perm)
+  (#_ : squash (SZ.fits (bm*bk + bm/tm*(bn/tn))))
+  (#_ : squash (SZ.fits (bk*bn + bm/tm*(bn/tn))))
+  (#_ : squash (rows/bm * (cols/bn) <= max_blocks
                /\ (bm/tm * (bn/tn)) <= max_threads))
+  ()
   : kernel_desc
       ((gA |-> Frac fA eA) ** (gB |-> Frac fB eB) ** (gC |-> eC))
       ((gA |-> Frac fA eA) ** (gB |-> Frac fB eB) ** (gC |-> MS.mmcomb comb eC eA eB))
 = {
-  nblk = mrows *^ mcols;
+  nblk = rows/^bm *^ (cols/^bn);
   nthr = (bm /^ tm *^ (bn /^ tn));
 
   shmems_desc = shmems_desc et bm bn bk;
 
   frame = emp;
-  block_pre  = (fun bid -> forall+ (tid : natlt (bm/^tm *^ (bn/^tn))). kpre1  comb tm tn gA gB gC eA eB fA fB bid tid);
-  block_post = (fun bid -> forall+ (tid : natlt (bm/^tm *^ (bn/^tn))). kpost1 comb tm tn gA gB gC eA eB fA fB bid tid);
-  setup      = setup    comb bm bn bk tm tn gA gB gC #eA #eB #eC;
-  teardown   = teardown comb bm bn bk tm tn gA gB gC #eA #eB #eC;
+  block_pre  = (fun bid -> forall+ (tid : natlt (bm/^tm *^ (bn/^tn))). kpre1  comb gA eA gB eB gC bm bn bk tm tn fA fB bid tid);
+  block_post = (fun bid -> forall+ (tid : natlt (bm/^tm *^ (bn/^tn))). kpost1 comb gA eA gB eB gC bm bn bk tm tn fA fB bid tid);
+  setup      = setup    comb gA eA gB eB gC eC bm bn bk tm tn fA fB;
+  teardown   = teardown comb gA eA gB eB gC eC bm bn bk tm tn fA fB;
 
   block_frame    = (fun _ar _bid -> emp);
-  block_setup    = block_setup comb bm bn bk tm tn slA slB gA gB gC #eA #eB #eC;
-  block_teardown = block_teardown comb bm bn bk tm tn slA slB gA gB gC #eA #eB #eC;
+  block_setup    = block_setup comb gA eA gB eB gC eC bm bn bk slA slB tm tn fA fB;
+  block_teardown = block_teardown comb gA eA gB eB gC eC bm bn bk slA slB tm tn fA fB ;
 
-  kpre      = kpre  comb tm tn slA slB gA gB gC eA eB fA fB;
-  kpost     = kpost comb tm tn slA slB gA gB gC eA eB fA fB;
+  kpre      = kpre  comb gA eA gB eB gC bm bn bk slA slB tm tn fA fB;
+  kpost     = kpost comb gA eA gB eB gC bm bn bk slA slB tm tn fA fB;
 
-  f = kf comb tm tn slA slB gA #fA gB #fB gC #eA #eB;
+  f = kf comb gA #eA gB #eB gC bm bn bk slA slB tm tn #() #() #fA #fB;
 }
 
+#push-options "--debug SMTFail --split_queries always"
 inline_for_extraction noextract
 fn mmcomb_gpu
   (#et : Type0) {| scalar et |}
   (comb : binop et)
-  (bm bn bk : szp)
-  (#mrows #mshared #mcols : szp)
+  (#rows #shared #cols : szp)
+  (#lA : mlayout rows shared)
+  (#lB : mlayout shared cols)
+  (#lC : mlayout rows cols)
+  {| clayout lA, clayout lB, clayout lC |}
+  (gA : gpu_matrix et lA)
+  (eA : ematrix et rows shared)
+  (gB : gpu_matrix et lB)
+  (eB : ematrix et shared cols)
+  (gC : gpu_matrix et lC)
+  (eC : ematrix et rows cols)
+  (bm : szp{bm /? rows})
+  (bn : szp{bn /? cols})
+  (bk : szp{bk /? shared})
   (tm : szp{tm /? bm})
   (tn : szp{tn /? bn})
   (#_ : squash (SZ.fits (bm*bk + bm/tm*(bn/tn))))
   (#_ : squash (SZ.fits (bk*bn + bm/tm*(bn/tn))))
+  (#_: squash (SZ.fits (bm * bk) /\ SZ.fits (bk * bn)))
   (slA : full_mlayout bm bk)
   (slB : full_mlayout bk bn)
   {| clayout slA, clayout slB |}
-  (lA : mlayout4 mrows   mshared bm bk)
-  (lB : mlayout4 mshared mcols   bk bn)
-  (lC : mlayout4 mrows   mcols   bm bn)
-  {| clayout4 lA, clayout4 lB, clayout4 lC |}
-  (gA : gpu_matrix4 et lA)
-  (#fA : perm)
-  (gB : gpu_matrix4 et lB)
-  (#fB : perm)
-  (gC : gpu_matrix4 et lC)
-  (#eA : ematrix4 et mrows mshared bm bk)
-  (#eB : ematrix4 et mshared mcols bk bn)
-  (#eC : ematrix4 et mrows mcols bm bn)
+  (fA fB : perm)
   preserves
     cpu **
     (gA |-> Frac fA eA) **
     (gB |-> Frac fB eB)
   requires
-    pure (mrows * mcols <= max_blocks) **
+    pure (rows/bm * (cols/bn) <= max_blocks) **
     pure (bm/tm * (bn/tn) <= max_threads) **
     (gC |-> eC)
   ensures
     gC |-> MS.mmcomb comb eC eA eB
 {
   (* fixed the inner layouts, or we'd have to propagate this everywhere? *)
-  launch_sync (mk_kernel comb bm bn bk tm tn slA slB gA gB gC ());
+  launch_sync (mk_kernel comb gA gB gC bm bn bk slA slB tm tn ());
 }
+
