src/lib/poly/gemm/Kuiper.Poly.GEMM.TensorCore.fst
@@ -4,9 +4,10 @@ module Kuiper.Poly.GEMM.TensorCore
 
 open Kuiper
 
+#set-options "--z3rlimit 20"
+
 module EM = Kuiper.EMatrix
 
-open Kuiper.EMatrix4
 open Kuiper.Matrix.Reprs.Type
 open Kuiper.Math { even, odd, even_2x, odd_2x1 }
 
@@ -38,45 +39,52 @@ let shmems_desc
   SHArray et (bk *^ bn);
 ]
 
+unfold
 let bid_y
-  (rows cols : sz)
-  (bm : szp{bm /? rows})
-  (bn : szp{bn /? cols})
-  (bid : natlt (rows/bm * (cols/bn)))
-  : GTot (natlt (rows/bm))
+  (rows cols : erased nat)
+  (bm : erased nat {bm > 0 /\ bm /? rows})
+  (bn : erased nat {bn > 0 /\ bn /? cols})
+  (bid : enatlt (rows/bm * (cols/bn)))
+  : enatlt (rows/bm)
   =
     bid / (cols/bn)
 
+unfold
 let bid_x
-  (rows cols : sz)
-  (bm : szp{bm /? rows})
-  (bn : szp{bn /? cols})
-  (bid : natlt (rows/bm * (cols/bn)))
-  : GTot (natlt (cols/bn))
+  (rows cols : erased nat)
+  (bm : erased nat {bm > 0 /\ bm /? rows})
+  (bn : erased nat {bn > 0 /\ bn /? cols})
+  (bid : enatlt (rows/bm * (cols/bn)))
+  : enatlt (cols/bn)
   =
   bid % (cols/bn)
 
+unfold
 let tid_y
-  (bm bn : sz)
-  (tm : szp{tm /? bm})
-  (tn : szp{tn /? bn})
-  (tid : natlt (bm/tm * (bn/tn)))
-  : GTot (natlt (bm/tm))
+  (bm bn : erased nat)
+  (tm : erased nat {tm > 0 /\ tm /? bm})
+  (tn : erased nat {tn > 0 /\ tn /? bn})
+  (tid : enatlt (bm/tm * (bn/tn)))
+  : enatlt (bm/tm)
   =
     tid / (bn/tn)
 
+unfold
 let tid_x
-  (bm bn : sz)
-  (tm : szp{tm /? bm})
-  (tn : szp{tn /? bn})
-  (tid : natlt (bm/tm * (bn/tn)))
-  : GTot (natlt (bn/tn))
+  (bm bn : erased nat)
+  (tm : erased nat {tm > 0 /\ tm /? bm})
+  (tn : erased nat {tn > 0 /\ tn /? bn})
+  (tid : enatlt (bm/tm * (bn/tn)))
+  : enatlt (bn/tn)
   =
     tid % (bn/tn)
 
+inline_for_extraction noextract
+instance concrete_sz_1 : concrete_sz 1 = { x = 1sz }
+
 let block_tile
   (#et : Type0) {| scalar et |}
-  (#rows #cols : sz)
+  (#rows #cols : erased nat)
   (#lC : mlayout rows cols)
   (gC : gpu_matrix et lC)
   (bm : szp{bm /? rows})
@@ -104,15 +112,15 @@ let thread_tile
 
 let own_thread_tile
   (#et : Type0) {| scalar et |}
-  (#rows #cols : sz)
+  (#rows #cols : erased nat)
   (#lC : mlayout rows cols)
   (gC : gpu_matrix et lC)
   (bm : szp{bm /? rows})
   (bn : szp{bn /? cols})
   (tm : szp{tm /? bm})
   (tn : szp{tn /? bn})
-  (bid : natlt ((rows/bm) * (cols/bn)))
-  (tid : natlt (bm/tm * (bn/tn)))
+  (bid : enatlt ((rows/bm) * (cols/bn)))
+  (tid : enatlt (bm/tm * (bn/tn)))
   : slprop
   = 
     (exists* em.
@@ -138,8 +146,8 @@ let kpre1
   (tm : szp{tm /? bm})
   (tn : szp{tn /? bn})
   (fA fB : perm)
-  (bid : natlt (rows/bm * (cols/bn)))
-  (tid : natlt (bm/tm * (bn/tn)))
+  (bid : enatlt (rows/bm * (cols/bn)))
+  (tid : enatlt (bm/tm * (bn/tn)))
   : slprop
   =
   (gA |-> Frac (fA /. (rows/tm * (cols/tn))) eA) **
@@ -165,8 +173,8 @@ let kpost1
   (tm : szp{tm /? bm})
   (tn : szp{tn /? bn})
   (fA fB : perm)
-  (bid : natlt (rows/bm * (cols/bn)))
-  (tid : natlt (bm/tm * (bn/tn)))
+  (bid : enatlt (rows/bm * (cols/bn)))
+  (tid : enatlt (bm/tm * (bn/tn)))
   : slprop
   =
   (gA |-> Frac (fA /. (rows/tm * (cols/tn))) eA) **
@@ -175,29 +183,30 @@ let kpost1
   
 let own_shmem_cell
   (#et : Type0)
-  (#rows #cols : nat)
+  (#rows #cols : erased nat)
   (#lm : mlayout rows cols)
   (sm : gpu_matrix et lm)
-  (i : natlt rows)
-  (j : natlt cols)
+  (i : enatlt rows)
+  (j : enatlt cols)
   : slprop
   = exists* v. gpu_matrix_pts_to_cell sm i j v
 
-let div_ceil (a : nat) (b : pos) = (a + (b-1))/b
+let div_ceil (a : erased nat) (b : pos) = (a + (b-1))/b
 let own_tile_stride_cells
   (#et : Type0)
-  (#rows #cols : nat)
+  (#rows #cols : erased nat)
   (#lm : mlayout rows cols)
   ([@@@mkey] m : gpu_matrix et lm)
   // (em : ematrix et rows cols)
-  (nthr : nat)
-  (tid : natlt nthr)
+  (nthr : erased nat)
+  (tid : enatlt nthr)
   : slprop
   =
+  (* using enatlt here would require enumerable enatlt which is not entirely straightforward *)
   forall+ (it : natlt (div_ceil (rows*cols) nthr)).
-    let flat_idx = tid + (it * nthr) <: nat in
-    let i = flat_idx/cols <: nat in
-    let j = flat_idx%cols <: nat in
+    let flat_idx = tid + (it * nthr) <: erased nat in
+    let i = flat_idx/cols <: erased nat in
+    let j = flat_idx%cols <: erased nat in
       if (i < rows && j < cols)
       then own_shmem_cell m i j
       else emp
@@ -301,7 +310,7 @@ let barrier_tok
   (l2 : full_mlayout bk bn)
   (sar1 : gpu_array et (bm * bk))
   (sar2 : gpu_array et (bk * bn))
-  (it : nat)
+  (it : erased nat)
   (nthr : pos)
   (tid : natlt nthr)
   : slprop
@@ -419,7 +428,7 @@ fn populate_shmem
   ();
 }
 
-#push-options "--debug SMTFail --split_queries always"
+// #push-options "--debug SMTFail --split_queries always --print_implicits"
 inline_for_extraction noextract
 fn subproducts2d
   (#et : Type0) {| scalar et |}
@@ -470,12 +479,6 @@ fn subproducts2d
   {
     open Pulse.Lib.Array;
 
-    gpu_matrix_tile gA tm 1;
-    let a_tile = gpu_matrix_subtile gA tm 1sz arow !dotIdx;
-    let va = gpu_matrix_read a_tile 0sz 0sz;
-    // let va = gpu_matrix_read #_ #_ #_ #_ #(c_subtile_layout l1 tm 1sz arow !dotIdx) a_tile 0sz 0sz;
-    admit();
-
     let mut i0 = 0sz;
     while (SZ.(!i0 <^ tm))
       invariant
@@ -483,15 +486,14 @@ fn subproducts2d
           (i0 |-> vi) **
           (rAcol |-> vrAcol)
     {
-      // let va = gpu_matrix_read #_ #_ #_ #_ #(c_subtile_layout l1 tm 1sz arow !dotIdx) a_tile 0sz 0sz;
+      (* get rid of a few non-linear arithmetic expressions *)
+      let a_tile = gpu_matrix_extract_tile' gA tm 1 arow !dotIdx;
       let va = gpu_matrix_read a_tile !i0 0sz;
+      ambig_trade_elim ();
       rAcol.(!i0) <- va;
 
       i0 := !i0 +^ 1sz;
     };
-
-    gpu_matrix_tile gB 1 tn;
-    let b_tile = gpu_matrix_subtile gB 1 tn !dotIdx bcol;
 
     let mut i1 = 0sz;
     while (SZ.(!i1 <^ tn))
@@ -500,7 +502,9 @@ fn subproducts2d
           (i1 |-> vi) **
           (rBrow |-> vrBrow)
     {
-      let vb = gpu_matrix_read b_tile !i1;
+      let b_tile = gpu_matrix_extract_tile' gB 1 tn !dotIdx bcol;
+      let vb = gpu_matrix_read b_tile 0sz !i1;
+      ambig_trade_elim ();
       rBrow.(!i1) <- vb;
 
       i1 := !i1 +^ 1sz;
@@ -520,6 +524,7 @@ fn subproducts2d
             (resIdxN |-> vresIdxN) **
             (rchProd |-> vrchProd)
       {
+        (* works on arrays and therefore does not have the nice matrix abstraction *)
         let ra = rAcol.(!resIdxM);
         let rb = rBrow.(!resIdxN);
         let iM = !resIdxM;
@@ -539,112 +544,77 @@ fn subproducts2d
   }
 }
 
-// inline_for_extraction noextract
-// fn subproducts_tc
-//   (* TODO restrict et to valid types only *)
-//   (#et : Type0) {| scalar et |}
-//   (bm bn bk: szp)
-//   (tm : szp{tm /? bm})
-//   (tn : szp{tn /? bn})
-//   (tk : szp{tk /? bk})
-//   (aFrag : fragment et FragA tm tn tk FragLCM)
-//   (#vaFrag : ematrix et tm tk)
-//   (bFrag : fragment et FragB tm tn tk FragLRM)
-//   (#vbFrag : ematrix et tk tn)
-//   (accumFrag : fragment et FragAccum tm tn tk FragLAccum)
-//   (#vaccumFrag : ematrix et tm tn)
-//   (#l1 : mlayout bm bk) {| clayout l1 |}
-//   (#l2 : mlayout bk bn) {| clayout l2 |}
-//   (gA : gpu_matrix et l1)
-//   (gB : gpu_matrix et l2)
-//   (#eA : ematrix et bm bk)
-//   (#eB : ematrix et bk bn)
-//   (#f : perm)
-//   (arow: szlt (bm/tm))
-//   (bcol : szlt (bn/tn))
-//   preserves
-//     gpu **
-//     (gA |-> Frac f eA) **
-//     (gB |-> Frac f eB)
-//   requires
-//     (aFrag |-> vaFrag) **
-//     (bFrag |-> vbFrag) **
-//     (accumFrag |-> vaccumFrag)
-//   ensures
-//     exists* vaFrag' vbFrag' vaccumFrag'.
-//       (aFrag |-> vaFrag') **
-//       (bFrag |-> vbFrag') **
-//       (accumFrag |-> vaccumFrag')
-// {
-//   let mut dotIdx : sz = 0sz;
-//   while (SZ.(!dotIdx <^ bk))
-//     invariant
-//       exists* (vdotIdx : sz{vdotIdx <= bk}) (vaFrag : ematrix et tm tk)
-//         (vbFrag : ematrix et tk tn) (vaccumFrag : ematrix et tm tn).
-//         (dotIdx |-> vdotIdx) **
-//         (aFrag |-> vaFrag) **
-//         (bFrag |-> vbFrag) **
-//         (accumFrag |-> vaccumFrag)
-//   {
+#push-options "--debug SMTFail --split_queries always"
+inline_for_extraction noextract
+fn subproducts_tc
+  (* TODO restrict et to valid types only *)
+  (#et : Type0) {| scalar et |}
+  (bm bn bk: szp)
+  (tm : szp{tm /? bm})
+  (tn : szp{tn /? bn})
+  (tk : szp{tk /? bk})
+  (* is FragLCM layout for aFrag relevant here? *)
+  (aFrag : fragment et FragA tm tn tk FragLRM)
+  (#vaFrag : ematrix et tm tk)
+  (bFrag : fragment et FragB tm tn tk FragLRM)
+  (#vbFrag : ematrix et tk tn)
+  (accumFrag : fragment et FragAccum tm tn tk FragLAccum)
+  (#vaccumFrag : ematrix et tm tn)
+  (gA : gpu_matrix et (R.row_major bm bk))
+  (gB : gpu_matrix et (R.row_major bk bn))
+  (#eA : ematrix et bm bk)
+  (#eB : ematrix et bk bn)
+  (#f : perm)
+  (arow: szlt (bm/tm))
+  (bcol : szlt (bn/tn))
+  preserves
+    gpu **
+    (gpu_matrix_pts_to gA #f eA) **
+    (gpu_matrix_pts_to gB #f eB)
+  requires
+    (aFrag |-> vaFrag) **
+    (bFrag |-> vbFrag) **
+    (accumFrag |-> vaccumFrag)
+  ensures
+    exists* vaFrag' vbFrag' vaccumFrag'.
+      (aFrag |-> vaFrag') **
+      (bFrag |-> vbFrag') **
+      (accumFrag |-> vaccumFrag')
+{
+  let mut dotIdx : sz = 0sz;
+  while (SZ.(!dotIdx <^ (bk/^tk)))
+    invariant
+      exists* (vdotIdx : sz{vdotIdx <= (bk/^tk)}) (vaFrag : ematrix et tm tk)
+        (vbFrag : ematrix et tk tn) (vaccumFrag : ematrix et tm tn).
+        (dotIdx |-> vdotIdx) **
+        (aFrag |-> vaFrag) **
+        (bFrag |-> vbFrag) **
+        (accumFrag |-> vaccumFrag)
+  {
+    let a_tile = gpu_matrix_extract_tile' gA tm tk arow !dotIdx;
+    mma_loadA aFrag a_tile;
+    let b_tile = gpu_matrix_extract_tile' gB tk tn !dotIdx bcol;
+    mma_loadB bFrag b_tile;
+    mma_sync' aFrag bFrag accumFrag;
 
-//     let mut i1 = 0sz;
-//     while (SZ.(!i1 <^ tn))
-//       invariant
-//         exists* (vi : sz{vi <= tn}) (vrBrow : erased (lseq et tn)).
-//           (i1 |-> vi) **
-//           (rBrow |-> vrBrow)
-//     {
-//       let vb = M.gpu_matrix_read gB !dotIdx (bcol *^ tn +^ !i1);
-//       rBrow.(!i1) <- vb;
-
-//       i1 := !i1 +^ 1sz;
-//     };
-
-//     let mut resIdxM = 0sz;
-//     while (SZ.(!resIdxM <^ tm))
-//       invariant
-//         exists* (vresIdxM : sz{vresIdxM <= tm}) (vrchProd : erased (lseq et (tm*tn))).
-//           (resIdxM |-> vresIdxM) **
-//           (rchProd |-> vrchProd)
-//     {
-//       let mut resIdxN = 0sz;
-//       while (SZ.(!resIdxN <^ tn))
-//         invariant
-//           exists* (vresIdxN : sz{vresIdxN <= tn}) (vrchProd : erased (lseq et (tm*tn))).
-//             (resIdxN |-> vresIdxN) **
-//             (rchProd |-> vrchProd)
-//       {
-//         let ra = rAcol.(!resIdxM);
-//         let rb = rBrow.(!resIdxN);
-//         let iM = !resIdxM;
-//         let iN = !resIdxN;
-//         assert(pure(SZ.fits(iM *^ tn +^ iN)));
-//         let old = rchProd.(!resIdxM *^ tn +^ !resIdxN);
-//         let mad = old `add` (ra `mul` rb);
-//         rchProd.(!resIdxM *^ tn +^ !resIdxN) <- mad;
-
-//         resIdxN := !resIdxN +^ 1sz;
-//       };
-
-//       resIdxM := !resIdxM +^ 1sz;
-//     };
-
-//     dotIdx := !dotIdx +^ 1sz;
-//   }
-// }
+    dotIdx := !dotIdx +^ 1sz;
+  }
+}
 
 inline_for_extraction noextract
 fn epilogue
   (#et : Type0) {| scalar et |}
   (comb : binop et)
-  (bm bn bk : szp)
-  (#rows #cols : szp)
+  (#rows #cols : sz)
+  (bm : szp{bm /? rows})
+  (bn : szp{bn /? cols})
   (tm : szp{tm /? bm})
   (tn : szp{tn /? bn})
   (rchProd: array et)
   (#lC : mlayout rows cols)
   {| clayout lC |}
   (gC : gpu_matrix et lC)
+  // (#_ : squash (SZ.fits (bm/tm * (bn/tn))))
   (bid : szlt (rows/bm * (cols/bn)))
   (tid : szlt (bm/tm * (bn/tn)))
   requires
@@ -661,59 +631,40 @@ fn epilogue
       (rchProd |-> vrchProd'))
 {
   unfold own_thread_tile gC bm bn tm tn bid tid;
-  let tt = thread_tile (block_tile gC bm bn bid) tm tn tid;
-  admit();
-  // let thread_tile = gpu_matrix_subtile
-
-  // let mrow = bid /^ mcols;
-  // let mcol = bid %^ mcols;
-  let tRowOff = tid /^ (bn /^ tn) *^ tm;
-  let tColOff = tid %^ (bn /^ tn) *^ tn;
+  let t_tile = thread_tile (block_tile gC bm bn bid) tm tn tid;
+  rewrite each thread_tile (block_tile gC bm bn bid) tm tn tid as t_tile;
+  // assert (rewrites_to t_tile (thread_tile (block_tile gC bm bn bid) tm tn tid));
 
   let mut resIdxM = 0sz;
   while (SZ.(!resIdxM <^ tm))
     invariant
-      exists* (vresIdxM : sz{vresIdxM <= tm}) (vrchProd : lseq et (tm*tn)).
+      exists* (vresIdxM : sz{vresIdxM <= tm}) (vrchProd : lseq et (tm*tn)) (v : ematrix et tm tn).
         (resIdxM |-> vresIdxM) **
-        (rchProd |-> vrchProd)
+        (rchProd |-> vrchProd) **
+        gpu_matrix_pts_to t_tile v
   {
     let mut resIdxN = 0sz;
     while (SZ.(!resIdxN <^ tn))
       invariant
-        exists* (vresIdxN : sz{vresIdxN <= tn}) (vrchProd : lseq et (tm*tn)).
+        exists* (vresIdxN : sz{vresIdxN <= tn}) (vrchProd : lseq et (tm*tn)) (v : ematrix et tm tn).
           (resIdxN |-> vresIdxN) **
-          (rchProd |-> vrchProd)
+          (rchProd |-> vrchProd) **
+          gpu_matrix_pts_to t_tile v
+
     {
-      let vresIdxM = !resIdxM;
-      let vresIdxN = !resIdxN;
-
-      (* get separate access to the thread's current cell in gC *)
-      forevery_extract_2 #(natlt tm) #_ #(natlt tn) (SZ.v vresIdxM) (SZ.v vresIdxN) _;
-
-      (* tame the SMT solver *)
-      assert pure(SZ.v tid / (SZ.v bn / SZ.v tn) * SZ.v tm == tRowOff);
-      assert pure(SZ.v tid % (SZ.v bn / SZ.v tn) * SZ.v tn == tColOff);
-
-      // assert pure (thread_row_offset bm bn tm tn tid vresIdxM == tid/(bn/tn)*tm + vresIdxM ==> tid/(bn/tn)*tm + vresIdxM < bm);
-      (* read the current cell in gC *)
-      with i0 j0 v0.
-      rewrite gpu_matrix_pts_to_cell gC i0 j0 v0
-          as gpu_matrix_pts_to_cell gC vresIdxM vresIdxN v0;
-      let v0 = gpu_matrix_read_cell gC vresIdxM vresIdxN;
+      let v0 = gpu_matrix_read t_tile !resIdxM !resIdxN;
 
       (* add the new result in the register cache to the value from gC and overwrite the the cell in gC *)
       open Pulse.Lib.Array;
+      // all obvious but without the asserts the next line fails
+      assert pure (SZ.fits (tm * tn));
+      assert pure (SZ.fits ((tm-1) * tn + tn));
+      with vrchProd. assert Pulse.Lib.Array.Core.pts_to rchProd vrchProd;
+      assert pure (Seq.length vrchProd == tm * tn);
       let v1 = rchProd.(!resIdxM *^ tn +^ !resIdxN);
       let v' = comb v0 v1;
-      gpu_matrix_write_cell gC vresIdxM vresIdxN v';
 
-      (* return separate access to the thread's current cell in gC *)
-      // rewrite each (SZ.v mrow) as (bid/mcols);
-      // rewrite each (SZ.v mcol) as (bid%mcols);
-      rewrite each (SZ.v tRowOff) as (tid/(bn/tn) * tm);
-      // rewrite each (tid/(bn/tn) * tm + (SZ.v vresIdxM)) as thread_row_offset bm bn tm tn tid (SZ.v vresIdxM);
-      rewrite each (SZ.v tColOff) as (tid%(bn/tn) * tn);
-      Pulse.Lib.Trade.elim_trade _ _;
+      gpu_matrix_write t_tile !resIdxM !resIdxN v';
 
       resIdxN := !resIdxN +^ 1sz;
     };
@@ -721,7 +672,8 @@ fn epilogue
     resIdxM := !resIdxM +^ 1sz;
   };
 
-  fold own_thread_tile bm bn tm tn gC bid tid;
+  rewrite each t_tile as thread_tile (block_tile gC bm bn bid) tm tn tid;
+  fold own_thread_tile gC bm bn tm tn bid tid;
   ()
 }
 
@@ -729,40 +681,42 @@ inline_for_extraction noextract
 fn kf
   (#et : Type0) {| scalar et |}
   (comb : binop et)
-  (#bm #bn #bk : szp)
-  (#mrows #mshared #mcols : szp)
+  (#rows #shared #cols : szp)
+  (#lA : mlayout rows shared)
+  (#lB : mlayout shared cols)
+  (#lC : mlayout rows cols)
+  {| clayout lA, clayout lB, clayout lC |}
+  (gA : gpu_matrix et lA)
+  (#eA : ematrix et rows shared)
+  (gB : gpu_matrix et lB)
+  (#eB : ematrix et shared cols)
+  (gC : gpu_matrix et lC)
+  (bm : szp{bm /? rows})
+  (bn : szp{bn /? cols})
+  (bk : szp{bk /? shared})
+  (#_: squash (SZ.fits (bm * bk) /\ SZ.fits (bk * bn)))
+  (slA : full_mlayout bm bk)
+  (slB : full_mlayout bk bn)
+  {| clayout slA, clayout slB |}
   (tm : szp{tm /? bm})
   (tn : szp{tn /? bn})
   (#_ : squash (SZ.fits (bm*bk + bm/tm*(bn/tn))))
   (#_ : squash (SZ.fits (bk*bn + bm/tm*(bn/tn))))
-  (slA : mlayout bm bk)
-  (slB : mlayout bk bn)
-  {| clayout slA, clayout slB |}
-  (#lA : mlayout4 mrows   mshared bm bk)
-  (#lB : mlayout4 mshared mcols   bk bn)
-  (#lC : mlayout4 mrows   mcols   bm bn)
-  {| clayout4 lA, clayout4 lB, clayout4 lC |}
-  (gA : gpu_matrix4 et lA)
-  (#fA : perm)
-  (gB : gpu_matrix4 et lB)
-  (#fB : perm)
-  (gC : gpu_matrix4 et lC)
-  (#eA : ematrix4 et mrows mshared bm bk)
-  (#eB : ematrix4 et mshared mcols bk bn)
+  (#fA #fB : perm)
   (sh : c_shmems (shmems_desc et bm bn bk))
-  (bid : szlt (mrows * mcols))
+  (bid : szlt (rows/bm * (cols/bn)))
   (tid : szlt (bm/tm * (bn/tn)))
   ()
   requires
     gpu **
-    kpre comb tm tn slA slB gA gB gC eA eB fA fB sh bid tid **
+    kpre comb gA eA gB eB gC bm bn bk slA slB tm tn fA fB sh bid tid **
     thread_id (bm/tm * (bn/tn)) tid **
-    block_id (mrows * mcols) bid
+    block_id (rows/bm * (cols/bn)) bid
   ensures
     gpu **
-    kpost comb tm tn slA slB gA gB gC eA eB fA fB sh bid tid **
+    kpost comb gA eA gB eB gC bm bn bk slA slB tm tn fA fB sh bid tid **
     thread_id (bm/tm * (bn/tn)) tid **
-    block_id (mrows * mcols) bid
+    block_id (rows/bm * (cols/bn)) bid
 {
   let sarA : gpu_array et (bm * bk) = fst sh;
   let sarB : gpu_array et (bk * bn) = fst (snd sh);
@@ -774,40 +728,43 @@ fn kf
 
   unfold barrier_tok slA slB sarA sarB 0 (bm/tm * (bn/tn)) tid;
 
-  M.gpu_matrix_abs' slA sarA;
-  let sA = M.from_array slA sarA;
-  rewrite each M.from_array slA sarA as sA;
+  gpu_matrix_abs' slA sarA;
+  let sA = from_array slA sarA;
+  rewrite each from_array slA sarA as sA;
 
-  M.gpu_matrix_abs' slB sarB;
-  let sB = M.from_array slB sarB;
-  rewrite each M.from_array slB sarB as sB;
+  gpu_matrix_abs' slB sarB;
+  let sB = from_array slB sarB;
+  rewrite each from_array slB sarB as sB;
 
-  let mrow = bid /^ mcols;
-  let mcol = bid %^ mcols;
+  let num_k_tiles = shared /^ bk;
+  let num_n_tiles = cols /^ bn;
+  let mrow = bid /^ num_n_tiles;
+  let mcol = bid %^ num_n_tiles;
+
   let threadRow = tid /^ (bn/^tn);
   let threadCol = tid %^ (bn/^tn);
 
-  (* tensor core fragments *)
-  let aFrag = __alloc_fragment et FragA tm tn tk FragLCM;
-  let bFrag = __alloc_fragment et FragB tm tn tk FragLRM;
-  let accumFrag = __alloc_fragment et FragAccum tm tn tk FragAccum;
-  fill_fragment accumFrag fill_value_zero;
+  // (* tensor core fragments *)
+  // let aFrag = __alloc_fragment et FragA tm tn tk FragLCM;
+  // let bFrag = __alloc_fragment et FragB tm tn tk FragLRM;
+  // let accumFrag = __alloc_fragment et FragAccum tm tn tk FragAccum;
+  // fill_fragment accumFrag fill_value_zero;
+  (* register caches *)
+  let mut rAcol : Pulse.Lib.Array.array et = [| zero #et #_ ; tm |];
+  let mut rBrow : Pulse.Lib.Array.array et = [| zero #et #_ ; tn |];
+  let mut rchProd : Pulse.Lib.Array.array et = [| zero #et #_ ; tm*^tn |];
 
-admit();
   let mut bkIdx  : sz = 0sz;
-  while (SZ.(!bkIdx <^ mshared))
-    invariant b.
-      exists* (vbkIdx : SZ.t{vbkIdx <= mshared}) (vrAcol : lseq et tm) (vrBrow : lseq et tn) (vrchProd : lseq et (tm*tn)).
-        pure (b == (SZ.v vbkIdx < mshared)) **
+  while (SZ.(!bkIdx <^ num_k_tiles))
+    invariant
+      exists* (vbkIdx : SZ.t{vbkIdx <= num_k_tiles}) (vrAcol : lseq et tm) (vrBrow : lseq et tn) (vrchProd : lseq et (tm*tn)).
         (bkIdx |-> vbkIdx) **
         (rAcol |-> vrAcol) **
         (rBrow |-> vrBrow) **
         (rchProd |-> vrchProd) **
-        (gA |-> Frac (fA /. (mrows * mcols * (bm/tm * (bn/tn)))) eA) **
-        (gB |-> Frac (fB /. (mrows * mcols * (bm/tm * (bn/tn)))) eB) **
-        (exists* (x : ematrix _ _ _). sA |-> Frac (1.0R /. (bm/tm * (bn/tn))) x) **
-        (exists* (x : ematrix _ _ _). sB |-> Frac (1.0R /. (bm/tm * (bn/tn))) x) **
-        B.barrier_tok (barrier_p sA sB (bm/tm * (bn/tn))) (barrier_q sA sB (bm/tm * (bn/tn))) (2 * vbkIdx) tid **
+        (exists* (x : ematrix _ _ _). sA |-> Frac (1.0R /. ((bm/tm*(bn/tn)))) x) **
+        (exists* (x : ematrix _ _ _). sB |-> Frac (1.0R /. ((bm/tm*(bn/tn)))) x) **
+        B.barrier_tok (barrier_p sA sB ((bm/tm*(bn/tn)))) (barrier_q sA sB ((bm/tm*(bn/tn)))) (2 * vbkIdx) tid **
         gpu
   {
     (* This assert should not be needed. I don't know what effect it even has. *)
@@ -848,48 +805,52 @@ admit();
     bkIdx := !bkIdx +^ 1sz;
   };
 
-  epilogue comb bm bn bk tm tn rchProd gC bid tid;
+  epilogue comb bm bn tm tn rchProd gC bid tid;
 
-  M.gpu_matrix_concr sA; rewrite each M.core sA as sarA;
-  M.gpu_matrix_concr sB; rewrite each M.core sB as sarB;
+  gpu_matrix_concr sA; rewrite each core sA as sarA;
+  gpu_matrix_concr sB; rewrite each core sB as sarB;
 
-  fold barrier_tok slA slB sarA sarB (2 * mshared) (bm/tm * (bn/tn)) tid;
+  fold barrier_tok slA slB sarA sarB (2 * num_k_tiles) (bm/tm * (bn/tn)) tid;
 
   rewrite each sarA as fst sh;
   rewrite each sarB as fst (snd sh);
   ()
 }
 
-
+#push-options "--z3rlimit 20"
 ghost
 fn setup
   (#et : Type0) {| scalar et |}
   (comb : binop et)
-  (bm bn bk : szp{SZ.fits (bm * bk) /\ SZ.fits (bk * bn)})
-  (#mrows #mshared #mcols : szp)
+  (#rows #shared #cols : szp)
+  (#lA : mlayout rows shared)
+  (#lB : mlayout shared cols)
+  (#lC : mlayout rows cols)
+  {| clayout lA, clayout lB, clayout lC |}
+  (gA : gpu_matrix et lA)
+  (eA : ematrix et rows shared)
+  (gB : gpu_matrix et lB)
+  (eB : ematrix et shared cols)
+  (gC : gpu_matrix et lC)
+  (eC : ematrix et rows cols)
+  (bm : szp{bm /? rows})
+  (bn : szp{bn /? cols})
+  (bk : szp{bk /? shared})
+  // (#_: squash (SZ.fits (bm * bk) /\ SZ.fits (bk * bn)))
+  (#_: squash (SZ.fits (bm * bn)))
+  (#_: squash (SZ.fits (rows * cols)))
   (tm : szp{tm /? bm})
   (tn : szp{tn /? bn})
-  (#lA : mlayout4 mrows   mshared bm bk)
-  (#lB : mlayout4 mshared mcols   bk bn)
-  (#lC : mlayout4 mrows   mcols   bm bn)
-  {| clayout4 lA, clayout4 lB, clayout4 lC |}
-  (gA : gpu_matrix4 et lA)
-  (#fA : perm)
-  (gB : gpu_matrix4 et lB)
-  (#fB : perm)
-  (gC : gpu_matrix4 et lC)
-  (#eA : ematrix4 et mrows mshared bm bk)
-  (#eB : ematrix4 et mshared mcols bk bn)
-  (#eC : ematrix4 et mrows mcols bm bn)
+  (fA fB : perm)
   ()
   requires
     (gA |-> Frac fA eA) **
     (gB |-> Frac fB eB) **
     (gC |-> eC)
   ensures
-    (forall+ (bid : natlt (mrows *^ mcols))
-             (tid : natlt (bm /^ tm *^ (bn /^ tn))).
-      kpre1 comb tm tn gA gB gC eA eB fA fB bid tid) **
+    (forall+ (bid : natlt (rows/^bm *^ (cols/^bn)))
+             (tid : natlt (bm/^tm *^ (bn/^tn))).
+      kpre1 comb gA eA gB eB gC bm bn bk tm tn fA fB bid tid) **
     emp (* frame *)
 {
   admit();
@@ -899,36 +860,40 @@ ghost
 fn block_setup
   (#et : Type0) {| scalar et |}
   (comb : binop et)
-  (bm bn bk : szp{SZ.fits (bm * bk) /\ SZ.fits (bk * bn)})
-  (#mrows #mshared #mcols : szp)
+  (#rows #shared #cols : szp)
+  (#lA : mlayout rows shared)
+  (#lB : mlayout shared cols)
+  (#lC : mlayout rows cols)
+  (gA : gpu_matrix et lA)
+  (eA : ematrix et rows shared)
+  (gB : gpu_matrix et lB)
+  (eB : ematrix et shared cols)
+  (gC : gpu_matrix et lC)
+  (eC : ematrix et rows cols)
+  (bm : szp{bm /? rows})
+  (bn : szp{bn /? cols})
+  (bk : szp{bk /? shared})
+  // (#_: squash (SZ.fits (bm * bk) /\ SZ.fits (bk * bn)))
+  (#_: squash (SZ.fits (bm * bn)))
+  (#_: squash (SZ.fits (rows * cols)))
+  (slA : full_mlayout bm bk)
+  (slB : full_mlayout bk bn)
+  {| clayout slA, clayout slB |}
   (tm : szp{tm /? bm})
   (tn : szp{tn /? bn})
-  (slA : mlayout bm bk)
-  (slB : mlayout bk bn)
-  (#lA : mlayout4 mrows   mshared bm bk)
-  (#lB : mlayout4 mshared mcols   bk bn)
-  (#lC : mlayout4 mrows   mcols   bm bn)
-  {| clayout4 lA, clayout4 lB, clayout4 lC |}
-  (gA : gpu_matrix4 et lA)
-  (#fA : perm)
-  (gB : gpu_matrix4 et lB)
-  (#fB : perm)
-  (gC : gpu_matrix4 et lC)
-  (#eA : ematrix4 et mrows mshared bm bk)
-  (#eB : ematrix4 et mshared mcols bk bn)
-  (#eC : ematrix4 et mrows mcols bm bn)
+  (fA fB : perm)
   (sh : c_shmems (shmems_desc et bm bn bk))
-  (bid : natlt (mrows *^ mcols))
+  (bid : natlt (rows/^bm *^ (cols/^bn)))
   ()
   requires
-    block_setup_tok (bm /^ tm *^ (bn /^ tn)) **
+    block_setup_tok (bm/^tm *^ (bn/^tn)) **
     live_c_shmems sh **
-    (forall+ (tid : natlt (bm/^tm *^ (bn /^ tn))).
-      kpre1 comb tm tn gA gB gC eA eB fA fB bid tid)
+    (forall+ (tid : natlt (bm/^tm *^ (bn/^tn))).
+      kpre1 comb gA eA gB eB gC bm bn bk tm tn fA fB bid tid)
   ensures
-    block_setup_tok (bm/^tm *^ (bn /^ tn)) **
-    (forall+ (tid : natlt (bm/^tm *^ (bn /^ tn))).
-      kpre comb tm tn slA slB gA gB gC eA eB fA fB sh bid tid) **
+    block_setup_tok (bm/^tm *^ (bn/^tn)) **
+    (forall+ (tid : natlt (bm/^tm *^ (bn/^tn))).
+      kpre comb gA eA gB eB gC bm bn bk slA slB tm tn fA fB sh bid tid) **
     emp (* frame *)
 {
   admit();
@@ -938,35 +903,39 @@ ghost
 fn block_teardown
   (#et : Type0) {| scalar et |}
   (comb : binop et)
-  (bm bn bk : szp{SZ.fits (bm * bk) /\ SZ.fits (bk * bn)})
-  (#mrows #mshared #mcols : szp)
+  (#rows #shared #cols : szp)
+  (#lA : mlayout rows shared)
+  (#lB : mlayout shared cols)
+  (#lC : mlayout rows cols)
+  (gA : gpu_matrix et lA)
+  (eA : ematrix et rows shared)
+  (gB : gpu_matrix et lB)
+  (eB : ematrix et shared cols)
+  (gC : gpu_matrix et lC)
+  (eC : ematrix et rows cols)
+  (bm : szp{bm /? rows})
+  (bn : szp{bn /? cols})
+  (bk : szp{bk /? shared})
+  // (#_: squash (SZ.fits (bm * bk) /\ SZ.fits (bk * bn)))
+  (#_: squash (SZ.fits (rows * cols)))
+  (#_: squash (SZ.fits (bm * bn)))
+  (slA : full_mlayout bm bk)
+  (slB : full_mlayout bk bn)
+  {| clayout slA, clayout slB |}
   (tm : szp{tm /? bm})
   (tn : szp{tn /? bn})
-  (slA : mlayout bm bk)
-  (slB : mlayout bk bn)
-  (#lA : mlayout4 mrows   mshared bm bk)
-  (#lB : mlayout4 mshared mcols   bk bn)
-  (#lC : mlayout4 mrows   mcols   bm bn)
-  {| clayout4 lA, clayout4 lB, clayout4 lC |}
-  (gA : gpu_matrix4 et lA)
-  (#fA : perm)
-  (gB : gpu_matrix4 et lB)
-  (#fB : perm)
-  (gC : gpu_matrix4 et lC)
-  (#eA : ematrix4 et mrows mshared bm bk)
-  (#eB : ematrix4 et mshared mcols bk bn)
-  (#eC : ematrix4 et mrows mcols bm bn)
+  (fA fB : perm)
   (sh : c_shmems (shmems_desc et bm bn bk))
-  (bid : natlt (mrows *^ mcols))
+  (bid : natlt (rows/^bm *^ (cols/^bn)))
   ()
   requires
-    (forall+ (tid : natlt (bm/^tm *^ (bn /^ tn))).
-      kpost comb tm tn slA slB gA gB gC eA eB fA fB sh bid tid) **
+    (forall+ (tid : natlt (bm/^tm *^ (bn/^tn))).
+      kpost comb gA eA gB eB gC bm bn bk slA slB tm tn fA fB sh bid tid) **
     emp (* frame *)
   ensures
     live_c_shmems sh **
-    (forall+ (tid : natlt (bm/^tm *^ (bn /^ tn))).
-      kpost1 comb tm tn gA gB gC eA eB fA fB bid tid)
+    (forall+ (tid : natlt (bm/^tm *^ (bn/^tn))).
+      kpost1 comb gA eA gB eB gC bm bn bk tm tn fA fB bid tid)
 {
   admit();
 }
@@ -975,27 +944,29 @@ ghost
 fn teardown
   (#et : Type0) {| scalar et |}
   (comb : binop et)
-  (bm bn bk : szp{SZ.fits (bm * bk) /\ SZ.fits (bk * bn)})
-  (#mrows #mshared #mcols : szp)
+  (#rows #shared #cols : szp)
+  (#lA : mlayout rows shared)
+  (#lB : mlayout shared cols)
+  (#lC : mlayout rows cols)
+  (gA : gpu_matrix et lA)
+  (eA : ematrix et rows shared)
+  (gB : gpu_matrix et lB)
+  (eB : ematrix et shared cols)
+  (gC : gpu_matrix et lC)
+  (eC : ematrix et rows cols)
+  (bm : szp{bm /? rows})
+  (bn : szp{bn /? cols})
+  (bk : szp{bk /? shared})
+  (#_: squash (SZ.fits (rows * cols)))
+  (#_: squash (SZ.fits (bm * bn)))
   (tm : szp{tm /? bm})
   (tn : szp{tn /? bn})
-  (#lA : mlayout4 mrows   mshared bm bk)
-  (#lB : mlayout4 mshared mcols   bk bn)
-  (#lC : mlayout4 mrows   mcols   bm bn)
-  {| clayout4 lA, clayout4 lB, clayout4 lC |}
-  (gA : gpu_matrix4 et lA)
-  (#fA : perm)
-  (gB : gpu_matrix4 et lB)
-  (#fB : perm)
-  (gC : gpu_matrix4 et lC)
-  (#eA : ematrix4 et mrows mshared bm bk)
-  (#eB : ematrix4 et mshared mcols bk bn)
-  (#eC : ematrix4 et mrows mcols bm bn)
+  (fA fB : perm)
   ()
   requires
-    (forall+ (bid : natlt (mrows *^ mcols))
-             (tid : natlt (bm /^ tm *^ (bn /^ tn))).
-      kpost1 comb tm tn gA gB gC eA eB fA fB bid tid) **
+    (forall+ (bid : natlt (rows/^bm *^ (cols/^bn)))
+             (tid : natlt (bm/^tm *^ (bn/^tn))).
+      kpre1 comb gA eA gB eB gC bm bn bk tm tn fA fB bid tid) **
     emp (* frame *)
   ensures
     (gA |-> Frac fA eA) **
@@ -1011,95 +982,102 @@ fn teardown
     // (fun (bid, tid) -> kpost1 comb tile gA gB gC eA eB 1.0R bid tid);
   admit();
 }
+#pop-options
 
 inline_for_extraction noextract
 let mk_kernel
   (#et : Type0) {| scalar et |}
   (comb : binop et)
-  (bm bn bk : szp)
-  (#mrows #mshared #mcols : szp)
+  (#rows #shared #cols : szp)
+  (#lA : mlayout rows shared)
+  (#lB : mlayout shared cols)
+  (#lC : mlayout rows cols)
+  {| clayout lA, clayout lB, clayout lC |}
+  (gA : gpu_matrix et lA)
+  (#eA : ematrix et rows shared)
+  (gB : gpu_matrix et lB)
+  (#eB : ematrix et shared cols)
+  (gC : gpu_matrix et lC)
+  (#eC : ematrix et rows cols)
+  (bm : szp{bm /? rows})
+  (bn : szp{bn /? cols})
+  (bk : szp{bk /? shared})
+  (#_: squash (SZ.fits (bm * bk) /\ SZ.fits (bk * bn)))
+  (slA : full_mlayout bm bk)
+  (slB : full_mlayout bk bn)
+  {| clayout slA, clayout slB |}
   (tm : szp{tm /? bm})
   (tn : szp{tn /? bn})
+  (#fA #fB : perm)
   (#_ : squash (SZ.fits (bm*bk + bm/tm*(bn/tn))))
   (#_ : squash (SZ.fits (bk*bn + bm/tm*(bn/tn))))
-  (slA : mlayout bm bk)
-  (slB : mlayout bk bn)
-  {| clayout slA, clayout slB |}
-  (#lA : mlayout4 mrows   mshared bm bk)
-  (#lB : mlayout4 mshared mcols   bk bn)
-  (#lC : mlayout4 mrows   mcols   bm bn)
-  {| clayout4 lA, clayout4 lB, clayout4 lC |}
-  (gA : gpu_matrix4 et lA)
-  (#fA : perm)
-  (gB : gpu_matrix4 et lB)
-  (#fB : perm)
-  (gC : gpu_matrix4 et lC)
-  (#eA : ematrix4 et mrows mshared bm bk)
-  (#eB : ematrix4 et mshared mcols bk bn)
-  (#eC : ematrix4 et mrows mcols bm bn)
-  (_ : squash (mrows * mcols <= max_blocks
+  (#_ : squash (rows/bm * (cols/bn) <= max_blocks
                /\ (bm/tm * (bn/tn)) <= max_threads))
+  ()
   : kernel_desc
       ((gA |-> Frac fA eA) ** (gB |-> Frac fB eB) ** (gC |-> eC))
       ((gA |-> Frac fA eA) ** (gB |-> Frac fB eB) ** (gC |-> MS.mmcomb comb eC eA eB))
 = {
-  nblk = mrows *^ mcols;
+  nblk = rows/^bm *^ (cols/^bn);
   nthr = (bm /^ tm *^ (bn /^ tn));
 
   shmems_desc = shmems_desc et bm bn bk;
 
   frame = emp;
-  block_pre  = (fun bid -> forall+ (tid : natlt (bm/^tm *^ (bn/^tn))). kpre1  comb tm tn gA gB gC eA eB fA fB bid tid);
-  block_post = (fun bid -> forall+ (tid : natlt (bm/^tm *^ (bn/^tn))). kpost1 comb tm tn gA gB gC eA eB fA fB bid tid);
-  setup      = setup    comb bm bn bk tm tn gA gB gC #eA #eB #eC;
-  teardown   = teardown comb bm bn bk tm tn gA gB gC #eA #eB #eC;
+  block_pre  = (fun bid -> forall+ (tid : natlt (bm/^tm *^ (bn/^tn))). kpre1  comb gA eA gB eB gC bm bn bk tm tn fA fB bid tid);
+  block_post = (fun bid -> forall+ (tid : natlt (bm/^tm *^ (bn/^tn))). kpost1 comb gA eA gB eB gC bm bn bk tm tn fA fB bid tid);
+  setup      = setup    comb gA eA gB eB gC eC bm bn bk tm tn fA fB;
+  teardown   = teardown comb gA eA gB eB gC eC bm bn bk tm tn fA fB;
 
   block_frame    = (fun _ar _bid -> emp);
-  block_setup    = block_setup comb bm bn bk tm tn slA slB gA gB gC #eA #eB #eC;
-  block_teardown = block_teardown comb bm bn bk tm tn slA slB gA gB gC #eA #eB #eC;
+  block_setup    = block_setup comb gA eA gB eB gC eC bm bn bk slA slB tm tn fA fB;
+  block_teardown = block_teardown comb gA eA gB eB gC eC bm bn bk slA slB tm tn fA fB ;
 
-  kpre      = kpre  comb tm tn slA slB gA gB gC eA eB fA fB;
-  kpost     = kpost comb tm tn slA slB gA gB gC eA eB fA fB;
+  kpre      = kpre  comb gA eA gB eB gC bm bn bk slA slB tm tn fA fB;
+  kpost     = kpost comb gA eA gB eB gC bm bn bk slA slB tm tn fA fB;
 
-  f = kf comb tm tn slA slB gA #fA gB #fB gC #eA #eB;
+  f = kf comb gA #eA gB #eB gC bm bn bk slA slB tm tn #() #() #fA #fB;
 }
 
+#push-options "--debug SMTFail --split_queries always"
 inline_for_extraction noextract
 fn mmcomb_gpu
   (#et : Type0) {| scalar et |}
   (comb : binop et)
-  (bm bn bk : szp)
-  (#mrows #mshared #mcols : szp)
+  (#rows #shared #cols : szp)
+  (#lA : mlayout rows shared)
+  (#lB : mlayout shared cols)
+  (#lC : mlayout rows cols)
+  {| clayout lA, clayout lB, clayout lC |}
+  (gA : gpu_matrix et lA)
+  (eA : ematrix et rows shared)
+  (gB : gpu_matrix et lB)
+  (eB : ematrix et shared cols)
+  (gC : gpu_matrix et lC)
+  (eC : ematrix et rows cols)
+  (bm : szp{bm /? rows})
+  (bn : szp{bn /? cols})
+  (bk : szp{bk /? shared})
   (tm : szp{tm /? bm})
   (tn : szp{tn /? bn})
   (#_ : squash (SZ.fits (bm*bk + bm/tm*(bn/tn))))
   (#_ : squash (SZ.fits (bk*bn + bm/tm*(bn/tn))))
-  (slA : mlayout bm bk)
-  (slB : mlayout bk bn)
+  (#_: squash (SZ.fits (bm * bk) /\ SZ.fits (bk * bn)))
+  (slA : full_mlayout bm bk)
+  (slB : full_mlayout bk bn)
   {| clayout slA, clayout slB |}
-  (lA : mlayout4 mrows   mshared bm bk)
-  (lB : mlayout4 mshared mcols   bk bn)
-  (lC : mlayout4 mrows   mcols   bm bn)
-  {| clayout4 lA, clayout4 lB, clayout4 lC |}
-  (gA : gpu_matrix4 et lA)
-  (#fA : perm)
-  (gB : gpu_matrix4 et lB)
-  (#fB : perm)
-  (gC : gpu_matrix4 et lC)
-  (#eA : ematrix4 et mrows mshared bm bk)
-  (#eB : ematrix4 et mshared mcols bk bn)
-  (#eC : ematrix4 et mrows mcols bm bn)
+  (fA fB : perm)
   preserves
     cpu **
     (gA |-> Frac fA eA) **
     (gB |-> Frac fB eB)
   requires
-    pure (mrows * mcols <= max_blocks) **
+    pure (rows/bm * (cols/bn) <= max_blocks) **
     pure (bm/tm * (bn/tn) <= max_threads) **
     (gC |-> eC)
   ensures
     gC |-> MS.mmcomb comb eC eA eB
 {
   (* fixed the inner layouts, or we'd have to propagate this everywhere? *)
-  launch_sync (mk_kernel comb bm bn bk tm tn slA slB gA gB gC ());
+  launch_sync (mk_kernel comb gA gB gC bm bn bk slA slB tm tn ());
 }
